bug in translation of Node corrected

src/ExpandWhens_rewritten.v
@@ -20,8 +20,6 @@ From mathcomp Require Import ssreflect ssrbool eqtype seq fintype ssrnat div ssr
 From simplssrlib Require Import SsrOrder Var FMaps.
 From firrtl Require Import Firrtl Env HiEnv HiFirrtl ModuleGraph_simplified.
 
-Section ExpandWhens.
-
 (* Precondition of ExpandWhens: all types that appear in the module
    are fully inferred, i.e. they are ground types, have no implicit
    width, and there is no abstract Freset type. *)
@@ -158,11 +156,13 @@ match s with
     | _, _ => false
     end
 | Smem _ m => if data_type m is Gtyp gt then fully_inferred gt else false
-| Sinvalid _ => true
+| Sinvalid r => ref_has_fully_inferred_ground_types r
 | Sinst _ _ => false (* instances are not supported currently *)
 | Snode _ e => expr_has_fully_inferred_ground_types e
-| Sfcnct _ e => expr_has_fully_inferred_ground_types e
-| Swhen _ ss_true ss_false =>
+| Sfcnct r e => ref_has_fully_inferred_ground_types r && expr_has_fully_inferred_ground_types e
+| Swhen cond ss_true ss_false =>
+       expr_has_fully_inferred_ground_types cond
+    &&
        stmts_have_fully_inferred_ground_types ss_true
     &&
        stmts_have_fully_inferred_ground_types ss_false
@@ -175,6 +175,22 @@ match ss with
     &&
        stmts_have_fully_inferred_ground_types ss'
 end.
+
+Lemma stmts_have_fully_inferred_ground_types_cat :
+forall (ss1 ss2 : HiFP.hfstmt_seq),
+    stmts_have_fully_inferred_ground_types ss1 ->
+        stmts_have_fully_inferred_ground_types ss2 ->
+            stmts_have_fully_inferred_ground_types (Qcat ss1 ss2).
+Proof.
+induction ss1 ; first by simpl Qcat ; done.
+intros.
+simpl stmts_have_fully_inferred_ground_types.
+simpl stmts_have_fully_inferred_ground_types in H.
+move /andP : H => H.
+rewrite (proj1 H) andTb.
+apply IHss1 ; last by exact H0.
+apply H.
+Qed.
 
 Lemma expr_preserves_fully_inferred :
 forall scope : CEP.t ftype,
@@ -242,11 +258,16 @@ Proof.
   + simpl ; trivial.
 Qed.
 
+Definition ct_has_fully_inferred_ground_types (ct : CEP.t def_expr) :=
+forall k : CEP.key, if CEP.find k ct is Some (D_fexpr e)
+                    then expr_has_fully_inferred_ground_types e
+                    else true.
+
 Lemma stmt_tmap_preserves_fully_inferred :
 forall (vm : CEP.t vertex_type) (tmap scope : CEP.t ftype) (s : HiFP.hfstmt),
    stmt_has_fully_inferred_ground_types s ->
    tmap_has_fully_inferred_ground_types tmap ->
-   submap scope tmap ->
+   CEP.submap scope tmap ->
       match stmt_tmap (tmap, scope) s vm with
       | Some (tmap', scope') => tmap_has_fully_inferred_ground_types tmap'
       | _ => True
@@ -255,7 +276,7 @@ with stmts_tmap_preserves_fully_inferred :
 forall (vm : CEP.t vertex_type) (ss : HiFP.hfstmt_seq) (tmap scope : CEP.t ftype),
    stmts_have_fully_inferred_ground_types ss ->
    tmap_has_fully_inferred_ground_types tmap ->
-   submap scope tmap ->
+   CEP.submap scope tmap ->
       match stmts_tmap (tmap, scope) ss vm with
       | Some (tmap', scope') => tmap_has_fully_inferred_ground_types tmap'
       | _ => True
@@ -305,7 +326,7 @@ Proof.
           specialize (H1 v).
           destruct (CEP.find v scope) ; try done.
           specialize (H0 v).
-          rewrite H1 in H0.
+          rewrite (H1 f Logic.eq_refl) in H0.
           by exact H0.
     simpl stmt_has_fully_inferred_ground_types in H.
     generalize (expr_preserves_fully_inferred scope H2 h H) ; intro.
@@ -329,7 +350,7 @@ Proof.
     simpl stmt_tmap.
     destruct (type_of_expr cond scope) ; last by done.
     simpl stmt_has_fully_inferred_ground_types in H.
-    move /andP : H => [Ht Hf].
+    move /andP : H => [/andP [_ Ht] Hf].
     generalize (stmts_tmap_preserves_fully_inferred vm ss_true tmap scope Ht H0 H1) ;
           intro.
     generalize (stmts_submap vm ss_true tmap scope H1) ;
@@ -338,8 +359,7 @@ Proof.
     specialize (stmts_tmap_preserves_fully_inferred vm ss_false tmap_true scope Hf H).
     destruct (stmts_tmap (tmap_true, scope) ss_false vm) as [[tmap_false _]|] ; try done.
     apply stmts_tmap_preserves_fully_inferred.
-    apply (submap_trans tmap) ; first by exact H1.
-    by apply H2.
+    by apply (CEP.Lemmas.submap_trans H1), H2.
 * clear stmts_tmap_preserves_fully_inferred.
   induction ss ; intros ; try done.
   simpl stmts_tmap.
@@ -352,6 +372,30 @@ Proof.
   destruct (stmts_tmap (tmap', scope') ss vm) as [[tmap'' _]|] ; by done.
 Qed.
 
+Lemma component_preserves_fully_inferred :
+forall (s : HiFP.hfstmt),
+    stmt_has_fully_inferred_ground_types s ->
+        stmts_have_fully_inferred_ground_types (component_stmt_of s)
+with components_preserves_fully_inferred :
+forall (ss : HiFP.hfstmt_seq),
+    stmts_have_fully_inferred_ground_types ss ->
+        stmts_have_fully_inferred_ground_types (component_stmts_of ss).
+Proof.
+* clear component_preserves_fully_inferred.
+  induction s ; simpl ; intros ; try done ; try rewrite andbT //.
+  rename h into cond ; rename h0 into ss_true ; rename h1 into ss_false.
+  move /andP : H => [/andP [_ Ht] Hf].
+  apply components_preserves_fully_inferred in Ht ;
+  apply components_preserves_fully_inferred in Hf.
+  apply stmts_have_fully_inferred_ground_types_cat ; assumption.
+* clear components_preserves_fully_inferred.
+  induction ss ; simpl ; intros ; try done.
+  move /andP : H => H.
+  apply stmts_have_fully_inferred_ground_types_cat.
+  * apply component_preserves_fully_inferred, H.
+  * apply IHss, H.
+Qed.
+
 Definition module_has_fully_inferred_ground_types (m : HiFP.hfmodule) : bool :=
 match m with
 | FInmod _ pp ss
@@ -360,6 +404,422 @@ match m with
     &&
        stmts_have_fully_inferred_ground_types ss
 end.
+
+(* Some helper properties of Sem *)
+Lemma fully_inferred_makes_Sem_frag_stmts_unique :
+forall (ss : HiFP.hfstmt_seq) (vm_old1 vm_old2 vm_new1 vm_new2 : CEP.t vertex_type)
+       (ct_old1 ct_old2 ct_new1 ct_new2 : CEP.t def_expr) (tmap : CEP.t ftype),
+    stmts_have_fully_inferred_ground_types ss ->
+    tmap_has_fully_inferred_ground_types tmap ->
+    CEP.Equal vm_old1 vm_old2 /\ CEP.Equal ct_old1 ct_old2 ->
+    Sem_frag_stmts vm_old1 ct_old1 ss vm_new1 ct_new1 tmap ->
+    Sem_frag_stmts vm_old2 ct_old2 ss vm_new2 ct_new2 tmap ->
+        CEP.Equal vm_new1 vm_new2 /\ CEP.Equal ct_new1 ct_new2
+with fully_inferred_makes_Sem_frag_stmt_unique :
+forall (s : HiFP.hfstmt) (vm_old1 vm_old2 vm_new1 vm_new2 : CEP.t vertex_type)
+       (ct_old1 ct_old2 ct_new1 ct_new2 : CEP.t def_expr) (tmap : CEP.t ftype),
+    stmt_has_fully_inferred_ground_types s ->
+    tmap_has_fully_inferred_ground_types tmap ->
+    CEP.Equal vm_old1 vm_old2 /\ CEP.Equal ct_old1 ct_old2 ->
+    Sem_frag_stmt vm_old1 ct_old1 s vm_new1 ct_new1 tmap ->
+    Sem_frag_stmt vm_old2 ct_old2 s vm_new2 ct_new2 tmap ->
+        CEP.Equal vm_new1 vm_new2 /\ CEP.Equal ct_new1 ct_new2.
+Proof.
+* clear fully_inferred_makes_Sem_frag_stmts_unique.
+  induction ss as [|s ss] ; simpl Sem_frag_stmts.
+  + split.
+    - apply CEP.Lemmas.Equal_trans with (m' := vm_old2) ; last by apply H3.
+      apply CEP.Lemmas.Equal_trans with (m' := vm_old1) ; last by apply H1.
+      by apply CEP.Lemmas.Equal_sym, H2.
+    - apply CEP.Lemmas.Equal_trans with (m' := ct_old2) ; last by apply H3.
+      apply CEP.Lemmas.Equal_trans with (m' := ct_old1) ; last by apply H1.
+      by apply CEP.Lemmas.Equal_sym, H2.
+  + intros.
+    simpl stmts_have_fully_inferred_ground_types in H ; move /andP : H => H.
+    destruct H2 as [vm_temp1 [ct_temp1 H2]].
+    destruct H3 as [vm_temp2 [ct_temp2 H3]].
+    specialize (fully_inferred_makes_Sem_frag_stmt_unique s
+                vm_old1 vm_old2 vm_temp1 vm_temp2
+                ct_old1 ct_old2 ct_temp1 ct_temp2 tmap
+                (proj1 H) H0 H1 (proj1 H2) (proj1 H3)).
+    specialize (IHss vm_temp1 vm_temp2 vm_new1 vm_new2
+                     ct_temp1 ct_temp2 ct_new1 ct_new2 tmap
+                     (proj2 H) H0 fully_inferred_makes_Sem_frag_stmt_unique
+                     (proj2 H2) (proj2 H3)).
+    exact IHss.
+* clear fully_inferred_makes_Sem_frag_stmt_unique.
+  destruct s ; simpl Sem_frag_stmt.
+  + (* Sskip *)
+    split.
+    - rewrite -(proj1 H2) -(proj1 H3) ; by apply H1.
+    - rewrite -(proj2 H2) -(proj2 H3) ; by apply H1.
+  + (* Swire *)
+    intros.
+    (*simpl stmt_has_fully_inferred_ground_types in H.*)
+    (*destruct f as [gt| |] ; try by done.*)
+    specialize (H0 s).
+    destruct (CEP.find s tmap) as [[gt'| |]|] ; try by done.
+    rewrite /list_rhs_type_p /size_of_ftype add1n in H2, H3.
+    split ; intro.
+    - destruct (y == s) eqn: Hys ; move /eqP : Hys => Hys.
+      * destruct H2 as [H2 _] ; destruct H3 as [H3 _].
+        specialize (H2 0) ; specialize (H3 0).
+        rewrite /List.nth_error add0n nat_of_binK -surjective_pairing in H2, H3.
+        by rewrite Hys (proj2 H2) (proj2 H3) //.
+      * destruct H2 as [_ [H2 _]] ; destruct H3 as [_ [H3 _]].
+        specialize (H2 y.1 y.2) ; specialize (H3 y.1 y.2).
+        rewrite -surjective_pairing in H2, H3.
+        destruct (N.eq_dec y.1 s.1) ;
+              last by (rewrite -H2 ; last (by left ; exact n) ;
+                       rewrite -H3 ; last (by left ; exact n) ;
+                       apply H1).
+        (* destruct (N.compare_spec y.2 s.2). --- Problem of this approach: the ``not equal'' cases are in %num scope, and I do not know how to change the scope *)
+        destruct (Nat.compare_spec y.2 s.2) ;
+              first (by apply (can_inj nat_of_binK) in H4 ;
+                        generalize (injective_projections y s e H4) ;
+                        contradiction) ;
+              move /ltP : H4 => H4.
+        + rewrite -H2 ; last (by right ; left ; exact H4) ;
+          rewrite -H3 ; last (by right ; left ; exact H4).
+          by apply H1.
+        + rewrite -H2 ; last (by right ; right ; exact H4) ;
+          rewrite -H3 ; last (by right ; right ; exact H4).
+          by apply H1.
+    - destruct (y == s) eqn: Hys ; move /eqP : Hys => Hys.
+      * destruct H2 as [_ [_ [_ H2]]] ; destruct H3 as [_ [_ [_ H3]]].
+        specialize (H2 0 (ltn0Sn 0)) ; specialize (H3 0 (ltn0Sn 0)).
+        rewrite add0n nat_of_binK -surjective_pairing in H2, H3.
+        by rewrite Hys H2 H3 //.
+      * destruct H2 as [_ [_ [H2 _]]] ; destruct H3 as [_ [_ [H3 _]]].
+        specialize (H2 y.1 y.2) ; specialize (H3 y.1 y.2).
+        rewrite -surjective_pairing in H2, H3.
+        destruct (N.eq_dec y.1 s.1) ;
+              last by (rewrite -H2 ; last (by left ; exact n) ;
+                       rewrite -H3 ; last (by left ; exact n) ;
+                       apply H1).
+        (* destruct (N.compare_spec y.2 s.2). --- Problem of this approach: the ``not equal'' cases are in %num scope, and I do not know how to change the scope *)
+        destruct (Nat.compare_spec y.2 s.2) ;
+              first (by apply (can_inj nat_of_binK) in H4 ;
+                        generalize (injective_projections y s e H4) ;
+                        contradiction) ;
+              move /ltP : H4 => H4.
+        + rewrite -H2 ; last (by right ; left ; exact H4) ;
+          rewrite -H3 ; last (by right ; left ; exact H4).
+          by apply H1.
+        + rewrite -H2 ; last (by right ; right ; exact H4) ;
+          rewrite -H3 ; last (by right ; right ; exact H4).
+          by apply H1.
+  + (* Sreg -- should be similar to Swire *)
+    admit.
+  + (* Smem -- not implemented *)
+    simpl ; by done.
+  + (* Sinst -- not implemented *)
+    simpl ; by done.
+  + (* Snode -- should be similar to Swire *)
+    admit.
+  + (* Sfcnct *)
+    intros.
+    destruct h0.
+    - (* Econst *)
+      simpl in H.
+      split ;
+            first (by destruct H2 as [H2 _] ; destruct H3 as [H3 _] ;
+                      apply CEP.Lemmas.Equal_trans with (m' := vm_old2) ; last (by exact H3) ;
+                      apply CEP.Lemmas.Equal_trans with (m' := vm_old1) ; last (by apply H1) ;
+                      apply CEP.Lemmas.Equal_sym, H2).
+      destruct H2 as [_ H2] ; destruct H3 as [_ H3].
+      generalize (list_lhs_ref_p_size tmap h) ; intro.
+      generalize (list_lhs_ref_p_type tmap h) ; intro.
+      destruct (type_of_ref h tmap) as [ft_ref|] ; last by contradiction H2.
+      destruct (type_of_expr (Econst ProdVarOrder.T f b) tmap) as [[ft_expr _]|] ; last by contradiction H2.
+      destruct H2 as [H6 H2] ; destruct H3 as [_ H3].
+      apply connect_type_compatible_size in H6.
+      destruct (list_lhs_ref_p h tmap) as [[input_list ft]|] ; last by contradiction H2.
+      rewrite H5 -H4 in H6 ; clear ft H4 H5.
+      generalize (list_rhs_expr_p_size ft_expr (Econst ProdVarOrder.T f b)) ; intro.
+      destruct (list_rhs_expr_p (Econst ProdVarOrder.T f b) ft_expr) as [expr_list|] ; last by contradiction H2.
+      rewrite -H6 in H4 ; clear H6.
+      intro.
+      destruct (y \in input_list) eqn: Hylist ;
+            last by (destruct H2 as [_ H2] ; destruct H3 as [_ H3] ;
+                     specialize (H2 y) ; specialize (H3 y) ;
+                     rewrite Hylist in H2, H3 ;
+                     rewrite -H2 -H3 ; apply H1).
+      destruct H2 as [H2 _] ; destruct H3 as [H3 _].
+      rewrite -index_mem in Hylist.
+      move /ltP : Hylist => Hylist.
+      generalize (proj2 (List.nth_error_Some input_list (index y input_list)) Hylist) ; intro.
+      specialize (H2 (index y input_list)) ; specialize (H3 (index y input_list)).
+      destruct (List.nth_error input_list (index y input_list)) as [ic|] eqn: H6 ; last by contradict H5.
+      clear H5.
+      replace ic with y in H2, H3, H6
+            by (clear -H6 ;
+                induction input_list ; first (by simpl in H6 ; done) ;
+                simpl in H6 ;
+                destruct (a == y) eqn: Hay ; simpl in H6 ;
+                      last (by apply IHinput_list, H6) ;
+                move /eqP : Hay => Hay ; rewrite Hay in H6 ;
+                symmetry ; injection H6 ; done).
+      clear ic.
+      rewrite -H4 in Hylist ; apply List.nth_error_Some in Hylist.
+      destruct (List.nth_error expr_list (index y input_list)) as [ex|] ; last by contradict Hylist.
+      by rewrite (proj2 H2) (proj2 H3) //.
+    - (* Ecast -- other expressions should be similar... *)
+      admit.
+    - (* Eprim_unop *)
+      admit.
+    - (* Eprim_binop *)
+      admit.
+    - (* Emux *)
+      admit.
+    - (* Evalidif *)
+      admit.
+    - (* Eref needs a slightly different treatment because it's bidirectional *)
+      admit.
+  + (* Sinvalid should be similar to Sfcnct but simpler *)
+    admit.
+  + (* Swhen -- use the induction hypotheses *)
+    admit.
+Admitted.
+
+
+Lemma Sem_frag_stmts_component_Equal :
+forall (ss : HiFP.hfstmt_seq) (vm_old1 vm_old2 : CEP.t vertex_type) (ct_old1 ct_old2 : CEP.t def_expr) (vm_new1 vm_new2 : CEP.t vertex_type) (ct_new : CEP.t def_expr) (tmap1 tmap2 : CEP.t ftype),
+    vm_and_ct_compatible vm_old1 ct_old1 ->
+    vm_and_ct_compatible vm_old2 ct_old2 ->
+    CEP.Equal vm_old1 vm_old2 ->
+    CEP.Equal vm_new1 vm_new2 ->
+    CEP.Equal tmap1 tmap2 ->
+    Sem_frag_stmts vm_old1 ct_old1 (component_stmts_of ss) vm_new1 ct_new tmap1 ->
+    Sem_frag_stmts vm_old2 ct_old2 (component_stmts_of ss) vm_new2 (extend_map_with ct_old2 ct_new) tmap2
+with Sem_frag_stmt_component_Equal :
+forall (s : HiFP.hfstmt) (vm_old1 vm_old2 : CEP.t vertex_type) (ct_old1 ct_old2 : CEP.t def_expr) (vm_new1 vm_new2 : CEP.t vertex_type) (ct_new : CEP.t def_expr) (tmap1 tmap2 : CEP.t ftype),
+    vm_and_ct_compatible vm_old1 ct_old1 ->
+    vm_and_ct_compatible vm_old2 ct_old2 ->
+    CEP.Equal vm_old1 vm_old2 ->
+    CEP.Equal vm_new1 vm_new2 ->
+    CEP.Equal tmap1 tmap2 ->
+    Sem_frag_stmts vm_old1 ct_old1 (component_stmt_of s) vm_new1 ct_new tmap1 ->
+    Sem_frag_stmts vm_old2 ct_old2 (component_stmt_of s) vm_new2 (extend_map_with ct_old2 ct_new) tmap2.
+Proof.
+* clear Sem_frag_stmts_component_Equal.
+  induction ss ; simpl ; intros.
+  + split.
+    - apply (CEP.Lemmas.Equal_trans (CEP.Lemmas.Equal_sym H1)).
+      exact (CEP.Lemmas.Equal_trans (proj1 H4) H2).
+    - intro ; rewrite /extend_map_with CEP.Lemmas.map2_1bis //.
+      specialize (H0 y).
+      destruct (CEP.find y ct_old2) ; first by reflexivity.
+      specialize (H y).
+      specialize (H1 y).
+      specialize (proj2 H4 y) ; intro.
+      destruct (CEP.find y vm_old2) as [[]|] ; try (by contradiction H0) ;
+            rewrite H1 H5 in H ; by rewrite H //.
+  + apply Sem_frag_stmts_cat.
+    apply Sem_frag_stmts_cat in H4.
+    destruct H4 as [vm_temp [ct_temp [H4 H5]]].
+    exists vm_temp, (extend_map_with ct_old2 ct_temp).
+    split.
+    - by apply (Sem_frag_stmt_component_Equal h vm_old1 vm_old2 ct_old1 ct_old2 vm_temp vm_temp ct_temp tmap1 tmap2
+                                              H H0 H1 (CEP.Lemmas.Equal_refl _) H3 H4).
+    - generalize (Sem_frag_stmts_compatible (component_stmt_of h) vm_old1 ct_old1 vm_temp ct_temp tmap1
+                                            H4) ; intro.
+      destruct H6 as [H6 [_ H7]] ; specialize (H7 H).
+      generalize (Sem_frag_stmts_component ss vm_temp ct_temp vm_new1 ct_new tmap1 H7 H5) ; intro.
+      generalize (extend_map_with_submap ct_old2 ct_temp ct_new H8) ; intro.
+      apply Sem_frag_stmts_Equal with (vm_old1 := vm_temp) (ct_old1 := extend_map_with ct_old2 ct_temp)
+                                      (vm_new1 := vm_new2) (ct_new1 := extend_map_with (extend_map_with ct_old2 ct_temp) ct_new)
+                                      (tmap1 := tmap2) ;
+            try assumption ; try apply CEP.Lemmas.Equal_refl.
+      apply IHss with (vm_old1 := vm_temp) (ct_old1 := ct_temp)
+                      (vm_new1 := vm_new1)
+                      (tmap1 := tmap1) ;
+            try assumption ; try apply CEP.Lemmas.Equal_refl.
+      generalize (Sem_frag_stmt_component h vm_old1 ct_old1 vm_temp ct_temp tmap1 H H4) ; intro.
+      intro.
+      specialize (H0 v) ; specialize (H1 v) ; specialize (H6 v) ;
+            rewrite H1 in H6.
+      rewrite CEP.Lemmas.map2_1bis //.
+      destruct (CEP.find v vm_old2) as [[]|] ;
+            try (by rewrite H0 ; apply H7) ;
+            by (rewrite (H6 _ Logic.eq_refl) ;
+                    destruct (CEP.find v ct_old2) ;
+                          first (by discriminate) ;
+                          last (by contradiction H0)).
+* clear Sem_frag_stmt_component_Equal.
+  destruct s ; intros.
+  + (* Sskip *)
+    simpl ; split ;
+        first by apply (CEP.Lemmas.Equal_trans (CEP.Lemmas.Equal_sym H1)),
+                       (CEP.Lemmas.Equal_trans (proj1 H4)), H2.
+    intro ; rewrite CEP.Lemmas.map2_1bis //.
+    specialize (H0 y).
+    destruct (CEP.find y ct_old2) ; first by reflexivity.
+    specialize (H1 y).
+    destruct (CEP.find y vm_old2) as [[]|] ;
+          try (by contradiction H0) ;
+          by (specialize (H y) ; rewrite H1 in H ;
+              specialize (proj2 H4 y) ; clear H4 ; intro H4 ;
+              rewrite -H4 H //).
+  + (* Swire *)
+    simpl ; simpl in H4.
+    destruct H4 as [vm' [ct' [H4 [H5 H6]]]].
+    exists vm_new2, (extend_map_with ct_old2 ct_new).
+    split ; last by split ; apply CEP.Lemmas.Equal_refl.
+    apply (CEP.Lemmas.Equal_trans) with (2 := H2) in H5.
+    clear H2 vm_new1.
+    specialize (H3 s).
+    destruct (CEP.find s tmap1) ; last by contradiction H4.
+    rewrite -H3 ; clear H3.
+    split.
+    - destruct H4 as [H4 _].
+      intro ; specialize (H4 n).
+      destruct (List.nth_error (list_rhs_type_p f0) n) ; last by trivial.
+      rewrite -H1 -H5.
+      exact H4.
+    split.
+    - destruct H4 as [_ [H4 _]].
+      intros v0 n0 ; specialize (H4 v0 n0).
+      rewrite -H1 -H5.
+      exact H4.
+    split.
+    - destruct H4 as [_ [_ [H4 _]]].
+      intros ; specialize (H4 v0 n0 H2).
+      rewrite CEP.Lemmas.map2_1bis // -H6.
+      specialize (H0 (v0, n0)).
+      destruct (CEP.find (v0, n0) ct_old2) ; first by reflexivity.
+      specialize (H1 (v0, n0)).
+      destruct (CEP.find (v0, n0) vm_old2) as [[]|] ;
+            try (by contradiction H0) ;
+            by (specialize (H (v0, n0)) ;
+                rewrite H1 in H ;
+                rewrite -H4 H //).
+    - destruct H4 as [H7 [_ [_ H4]]].
+      intros ; specialize (H4 n0 H2) ; specialize (H7 n0).
+      rewrite -(list_rhs_type_p_size f0) in H2.
+      move /ltP : H2 => H2.
+      generalize (proj2 (List.nth_error_Some (list_rhs_type_p f0) n0) H2) ; intro.
+      destruct (List.nth_error (list_rhs_type_p f0) n0) ; last by contradiction H3.
+      rewrite H1 in H7.
+      specialize (H0 (s.1, bin_of_nat (n0 + s.2))).
+      rewrite (proj1 H7) in H0.
+      rewrite CEP.Lemmas.map2_1bis // H0 -H6 H4 //.
+  + (* Sreg, should be similar to Swire *)
+    admit.
+  + (* Smem, TBD *)
+    simpl in H4.
+    destruct H4 as [_ [_ [H4 _]]].
+    contradiction H4.
+  + (* Sinst, TBD *)
+    simpl in H4.
+    destruct H4 as [_ [_ [H4 _]]].
+    contradiction H4.
+  + (* Snode, should be similar to Swire *)
+    admit.
+  + (* Sfcnct, similar to Sskip *)
+    simpl ; split ;
+        first by apply (CEP.Lemmas.Equal_trans (CEP.Lemmas.Equal_sym H1)),
+                       (CEP.Lemmas.Equal_trans (proj1 H4)), H2.
+    intro ; rewrite CEP.Lemmas.map2_1bis //.
+    specialize (H0 y).
+    destruct (CEP.find y ct_old2) ; first by reflexivity.
+    specialize (H1 y).
+    destruct (CEP.find y vm_old2) as [[]|] ;
+          try (by contradiction H0) ;
+          by (specialize (H y) ; rewrite H1 in H ;
+              specialize (proj2 H4 y) ; clear H4 ; intro H4 ;
+              rewrite -H4 H //).
+  + (* Sinvalid, similar to Sskip *)
+    simpl ; split ;
+        first by apply (CEP.Lemmas.Equal_trans (CEP.Lemmas.Equal_sym H1)),
+                       (CEP.Lemmas.Equal_trans (proj1 H4)), H2.
+    intro ; rewrite CEP.Lemmas.map2_1bis //.
+    specialize (H0 y).
+    destruct (CEP.find y ct_old2) ; first by reflexivity.
+    specialize (H1 y).
+    destruct (CEP.find y vm_old2) as [[]|] ;
+          try (by contradiction H0) ;
+          by (specialize (H y) ; rewrite H1 in H ;
+              specialize (proj2 H4 y) ; clear H4 ; intro H4 ;
+              rewrite -H4 H //).
+  + (* Swhen *)
+    rename h into cond ; rename h0 into ss_true ; rename h1 into ss_false.
+    simpl component_stmt_of in H4 ; simpl component_stmt_of.
+    apply Sem_frag_stmts_cat in H4 ; apply Sem_frag_stmts_cat.
+    destruct H4 as [vm_temp [ct_temp [H4 H5]]].
+    exists vm_temp, (extend_map_with ct_old2 ct_temp).
+    split.
+    - by apply (Sem_frag_stmts_component_Equal ss_true vm_old1 vm_old2 ct_old1 ct_old2 vm_temp vm_temp ct_temp tmap1 tmap2
+                                              H H0 H1 (CEP.Lemmas.Equal_refl _) H3 H4).
+    - generalize (Sem_frag_stmts_compatible (component_stmts_of ss_true) vm_old1 ct_old1 vm_temp ct_temp tmap1
+                                            H4) ; intro.
+      destruct H6 as [H6 [_ H7]] ; specialize (H7 H).
+      generalize (Sem_frag_stmts_component ss_false vm_temp ct_temp vm_new1 ct_new tmap1 H7 H5) ; intro.
+      generalize (extend_map_with_submap ct_old2 ct_temp ct_new H8) ; intro.
+      apply Sem_frag_stmts_Equal with (vm_old1 := vm_temp) (ct_old1 := extend_map_with ct_old2 ct_temp)
+                                      (vm_new1 := vm_new2) (ct_new1 := extend_map_with (extend_map_with ct_old2 ct_temp) ct_new)
+                                      (tmap1 := tmap2) ;
+            try assumption ; try apply CEP.Lemmas.Equal_refl.
+      apply Sem_frag_stmts_component_Equal with (vm_old1 := vm_temp) (ct_old1 := ct_temp)
+                      (vm_new1 := vm_new1)
+                      (tmap1 := tmap1) ;
+            try assumption ; try apply CEP.Lemmas.Equal_refl.
+      generalize (Sem_frag_stmts_component ss_true vm_old1 ct_old1 vm_temp ct_temp tmap1 H H4) ; intro.
+      intro.
+      specialize (H0 v) ; specialize (H1 v) ; specialize (H6 v) ;
+            rewrite H1 in H6.
+      rewrite CEP.Lemmas.map2_1bis //.
+      destruct (CEP.find v vm_old2) as [[]|] ;
+            try (by rewrite H0 ; apply H7) ;
+            by (rewrite (H6 _ Logic.eq_refl) ;
+                    destruct (CEP.find v ct_old2) ;
+                          first (by discriminate) ;
+                          last (by contradiction H0)).
+Admitted.
+
+Lemma Sem_frag_stmts_no_component :
+(* Only component statements change vm *)
+forall (ss : HiFP.hfstmt_seq) (vm_old vm_new : CEP.t vertex_type)
+       (ct_old ct_new : CEP.t def_expr) (tmap : CEP.t ftype),
+component_stmts_of ss = (Qnil ProdVarOrder.T) ->
+    Sem_frag_stmts vm_old ct_old ss vm_new ct_new tmap ->
+           CEP.Equal vm_old vm_new
+with Sem_frag_stmt_no_component :
+forall (s : HiFP.hfstmt) (vm_old vm_new : CEP.t vertex_type)
+       (ct_old ct_new : CEP.t def_expr) (tmap : CEP.t ftype),
+component_stmt_of s = (Qnil ProdVarOrder.T) ->
+    Sem_frag_stmt vm_old ct_old s vm_new ct_new tmap ->
+           CEP.Equal vm_old vm_new.
+Proof.
+* clear Sem_frag_stmts_no_component.
+  induction ss ; simpl Sem_frag_stmts ; intros ; first by apply H0.
+  simpl component_stmts_of in H ; apply Qcat_nil in H.
+  destruct H0 as [vm' [ct' H0]].
+  specialize (Sem_frag_stmt_no_component h vm_old vm' ct_old ct' tmap (proj1 H) (proj1 H0)).
+  specialize (IHss vm' vm_new ct' ct_new tmap (proj2 H) (proj2 H0)).
+  intro.
+  specialize (Sem_frag_stmt_no_component y) ; rewrite Sem_frag_stmt_no_component.
+  apply IHss.
+* clear Sem_frag_stmt_no_component.
+  induction s ; simpl component_stmt_of ; try discriminate ;
+  simpl Sem_frag_stmt ; intros.
+  + (* Sskip *)
+    rewrite (proj1 H0) ; reflexivity.
+  + (* Sfcnct *)
+    destruct h0 ; by apply H0.
+  + (* Sinvalid *)
+    by apply H0.
+  + (* Swhen *)
+    rename h into cond ; rename h0 into ss_true ; rename h1 into ss_false.
+    destruct (type_of_expr cond tmap) as [[[[[|[|]]| | | | | |]| |] _]|] ; try by contradiction H0.
+    apply Qcat_nil in H.
+    destruct H0 as [vm_true [ct_true [ct_false [Ht [Hf H0]]]]].
+    generalize (Sem_frag_stmts_no_component ss_true vm_old vm_true ct_old ct_true tmap (proj1 H) Ht) ; intro.
+    specialize (Sem_frag_stmts_no_component ss_false vm_true vm_new (extend_map_with ct_old ct_true) ct_false tmap (proj2 H) Hf).
+    intro.
+    specialize (H1 y) ; rewrite H1.
+    apply Sem_frag_stmts_no_component.
+Qed.
 
 (* We first define ExpandBranch_fun.
    It uses a map to indicate which expressions are connected in which
@@ -464,14 +924,14 @@ match s with
 | Sinst _ _ => None (* instances are not supported currently *)
 | Snode v e =>
     if type_of_expr e old_scope is Some (exist ft_expr _)
-    then Some (Qrcons old_def_ss s, CEP.add v (D_fexpr e) old_conn_map, CEP.add v ft_expr old_scope)
+    then Some (Qrcons old_def_ss s, old_conn_map, CEP.add v ft_expr old_scope)
     else None
 | Sfcnct ref e =>
     ExpandBranch_connect ref (D_fexpr e) old_def_ss old_conn_map old_scope
 | Swhen c ss_true ss_false =>
     match type_of_expr c old_scope, ExpandBranch_funs ss_true old_def_ss old_conn_map old_scope with
     | Some (exist (Gtyp (Fuint 1)) _), Some (true_def_ss, true_conn_map, _) =>
-        match ExpandBranch_funs ss_false true_def_ss old_conn_map old_scope with
+        match ExpandBranch_funs ss_false true_def_ss (extend_map_with old_conn_map true_conn_map) old_scope with
         | None => None
         | Some (false_def_ss, false_conn_map, _) =>
             Some (false_def_ss, CEP.map2 (helper_tf c) true_conn_map false_conn_map, old_scope)
@@ -566,17 +1026,12 @@ with ExpandBranch_component :
           def_ss' = Qcat def_ss (component_stmt_of s).
 Proof.
 * clear ExpandBranch_components.
-  induction ss.
-  + intros.
-    unfold ExpandBranch_funs in H.
-    unfold component_stmts_of.
-    rewrite Qcats0.
+  induction ss ; intros ; simpl ExpandBranch_funs in H ; simpl component_stmts_of.
+  + rewrite Qcats0.
     symmetry.
     injection H.
     by trivial.
-  + intros.
-    simpl ExpandBranch_funs in H ; simpl component_stmts_of.
-    specialize ExpandBranch_component with (s := h) (def_ss := def_ss) (conn_map := conn_map) (scope := scope).
+  + specialize ExpandBranch_component with (s := h) (def_ss := def_ss) (conn_map := conn_map) (scope := scope).
     destruct (ExpandBranch_fun h def_ss conn_map scope) as [[[def_ss0 conn_map0] scope0]|] ; last by discriminate H.
     specialize ExpandBranch_component with (def_ss' := def_ss0) (conn_map' := conn_map0) (scope' := scope0).
     apply IHss in H.
@@ -656,163 +1111,38 @@ Proof.
     destruct (ExpandBranch_funs ss_true def_ss conn_map scope) as [[[def_ss_true conn_map_true] scope_true]|] ; last by discriminate H.
     specialize (H0 def_ss_true conn_map_true scope_true Logic.eq_refl).
     simpl fst in H.
-    generalize (ExpandBranch_components ss_false def_ss_true conn_map scope) ;
+    generalize (ExpandBranch_components ss_false def_ss_true (extend_map_with conn_map conn_map_true) scope) ;
           intro.
-    destruct (ExpandBranch_funs ss_false def_ss_true conn_map scope) as [[[def_ss_false conn_map_false] scope_false]|] ; last by discriminate H.
+    destruct (ExpandBranch_funs ss_false def_ss_true (extend_map_with conn_map conn_map_true) scope) as [[[def_ss_false conn_map_false] scope_false]|] ; last by discriminate H.
     specialize (H1 def_ss_false conn_map_false scope_false Logic.eq_refl).
     unfold fst, snd in H ; injection H ; intros.
     rewrite -Qcat_assoc -H0 -H1 H4 //.
 Qed.
 
-(* The following is a nice lemma
-   but the subset old_scope1 old_scope2 is the wrong way round.
-   After this comes a lemma with the subsets the other way round;
-   note that the proofs are almost literally the same.
 
 Lemma ExpandBranch_stmt_tmap :
+(* When comparing stmt_tmap and ExpandBranch_fun:
+   if the first function gets a larger scope as input,
+   it will produce a larger scope as output.
+
+   This lemma is used by the next theorem (ExpandBranch_funs_checks_scopes). *)
 forall (vm : CEP.t vertex_type) (s : HiFP.hfstmt)
        (old_tmap new_tmap old_scope1 new_scope1 old_scope2 new_scope2 : CEP.t ftype)
        (old_def_ss new_def_ss : HiFP.hfstmt_seq) (old_conn_map new_conn_map : CEP.t def_expr),
    stmt_tmap (old_tmap, old_scope1) s vm = Some (new_tmap, new_scope1) ->
    ExpandBranch_fun s old_def_ss old_conn_map old_scope2 = Some (new_def_ss, new_conn_map, new_scope2) ->
-   submap old_scope1 old_scope2 ->
+   CEP.submap old_scope2 old_scope1 ->
    stmt_has_fully_inferred_ground_types s ->
-      submap new_scope1 new_scope2
+      CEP.submap new_scope2 new_scope1
 with ExpandBranch_stmts_tmap :
 forall (vm : CEP.t vertex_type) (ss : HiFP.hfstmt_seq)
        (old_tmap new_tmap old_scope1 new_scope1 old_scope2 new_scope2 : CEP.t ftype)
        (old_def_ss new_def_ss : HiFP.hfstmt_seq) (old_conn_map new_conn_map : CEP.t def_expr),
    stmts_tmap (old_tmap, old_scope1) ss vm = Some (new_tmap, new_scope1) ->
    ExpandBranch_funs ss old_def_ss old_conn_map old_scope2 = Some (new_def_ss, new_conn_map, new_scope2) ->
-   submap old_scope1 old_scope2 ->
+   CEP.submap old_scope2 old_scope1 ->
    stmts_have_fully_inferred_ground_types ss ->
-      submap new_scope1 new_scope2.
-Proof.
-* clear ExpandBranch_stmt_tmap.
-  destruct s ; simpl stmt_tmap ; simpl ExpandBranch_fun ; simpl stmt_has_fully_inferred_ground_types ; intros.
-  + (* Sskip *)
-    injection H ; clear H ; intros H _.
-    injection H0 ; clear H0 ; intros H0 _ _.
-    rewrite -H -H0.
-    by exact H1.
-  + (* Swire *)
-    injection H0 ; clear H0 ; intros H0 _ _.
-    rewrite -H0 ; clear H0 new_scope2.
-    destruct f as [gt| |] ; try done.
-    destruct (CEP.find s old_tmap) ; first by discriminate H.
-    generalize (fully_inferred_does_not_change gt s vm H2) ;
-          intro.
-    destruct (code_type_find_vm_widths (Gtyp gt) s vm) as [[[newgt| |] _]|]; try done.
-    rewrite -H0 in H ; clear H0 newgt.
-    injection H ; clear H ; intros H _.
-    rewrite -H ; clear H new_scope1.
-    apply submap_add_add, H1.
-  + (* Sreg *)
-    destruct (type h) as [gt| |] ; try done.
-    destruct (CEP.find s old_tmap) ; first by discriminate H.
-    destruct (type_of_expr (clock h) old_scope1) ; last by discriminate H.
-    destruct (reset h) as [|rst_sig rst_val].
-    1,2: move /andP : H2 => [_ H2].
-    1,2: generalize (fully_inferred_does_not_change gt s vm H2) ;
-          intro.
-    1,2: destruct (code_type_find_vm_widths (Gtyp gt) s vm) as [[[newgt| |] _]|] ; try done.
-    1,2: rewrite -H3 in H ; clear H3 newgt.
-    2: destruct (type_of_expr rst_sig old_scope1) ; last by discriminate H.
-    2: destruct (type_of_expr rst_val old_scope1) ; last by discriminate H.
-    2: destruct (type_of_expr rst_sig old_scope2) ; last by discriminate H0.
-    2: destruct (type_of_expr rst_val old_scope2) ; last by discriminate H0.
-    1,2: injection H ; clear H ; intros H _ ; rewrite -H ; clear H new_scope1.
-    1,2: destruct (type_of_expr (clock h) old_scope2) ; last by discriminate H0.
-    1,2: injection H0 ; clear H0 ; intros H0 _ _ ; rewrite -H0 ; clear H0 new_scope2.
-    1,2: apply submap_add_add, H1.
-  + (* Smem *)
-    by discriminate H.
-  + (* Sinst *)
-    by discriminate H.
-  + (* Snode *)
-    destruct (CEP.find s old_tmap) ; first by discriminate H.
-    generalize (type_of_expr_submap h old_scope1 old_scope2 H1) ;
-          intro.
-    destruct (type_of_expr h old_scope1) as [[ft1 p1]|] ; last by discriminate H.
-    destruct (type_of_expr h old_scope2) as [[ft2 p2]|] ; last by discriminate H0.
-    injection H3 ; clear H3 ; intro H3 ; rewrite H3 in H0 ; clear H3 p2 p1 ft2.
-    injection H ; clear H ; intros H _ ; rewrite -H ; clear H new_scope1.
-    injection H0 ; clear H0 ; intros H0 _ _ ; rewrite -H0 ; clear H0 new_scope2.
-    apply submap_add_add, H1.
-  + (* Sfcnct *)
-    unfold ExpandBranch_connect in H0.
-    destruct (type_of_ref h old_scope1) ; last by discriminate H.
-    destruct (type_of_expr h0 old_scope1) ; last by discriminate H.
-    injection H ; clear H ; intros H _ ; rewrite -H ; clear H new_scope1.
-    destruct h ; try done.
-    - destruct (CEP.find s old_scope2) ; last by discriminate H0.
-      destruct (type_of_expr h0 old_scope2) as [[ft_expr _]|] ; last by discriminate H0.
-      destruct (connect_type_compatible false f1 ft_expr false) ; last by discriminate H0.
-      injection H0 ; clear H0 ; intros H0 _ _ ; rewrite -H0 ; clear H0 new_scope2.
-      by exact H1.
-    - destruct h ; try done.
-      destruct h ; by done.
-  + (* Sinvalid *)
-    unfold ExpandBranch_connect in H0.
-    destruct (type_of_ref h old_scope1) ; last by discriminate H.
-    injection H ; clear H ; intros H _ ; rewrite -H ; clear H new_scope1.
-    destruct h ; try done.
-    - destruct (CEP.find s old_scope2) ; last by discriminate H0.
-      injection H0 ; clear H0 ; intros H0 _ _ ; rewrite -H0 ; clear H0 new_scope2.
-      by exact H1.
-    - destruct h ; try done.
-      destruct h ; by done.
-  + (* Swhen *)
-    rename h into cond ; rename h0 into ss_true ; rename h1 into ss_false.
-    destruct (type_of_expr cond old_scope1) ; last by discriminate H.
-    destruct (type_of_expr cond old_scope2) as [[[[[|[|]]| | | | | |]| |] _]|] ; try by discriminate H0.
-    destruct (stmts_tmap (old_tmap, old_scope1) ss_true vm) as [[tmap_true scope1_true]|] ; last by discriminate H.
-    destruct (ExpandBranch_funs ss_true old_def_ss old_conn_map old_scope2) as [[[true_def_ss true_conn_map] true_scope2]|] ; last by discriminate H0.
-    destruct (stmts_tmap (tmap_true, old_scope1) ss_false vm) as [[tmap_false scope1_false]|] ; last by discriminate H.
-    injection H ; clear H ; intros H _ ; rewrite -H ; clear H new_scope1.
-    destruct (ExpandBranch_funs ss_false true_def_ss old_conn_map old_scope2) as [[[false_def_ss false_conn_map] false_scope2]|] ; last by discriminate H0.
-    injection H0 ; clear H0 ; intros H0 _ _ ; rewrite -H0 ; clear H0 new_scope2.
-    by exact H1.
-* clear ExpandBranch_stmts_tmap.
-  induction ss.
-  + simpl stmts_tmap ; simpl ExpandBranch_funs ; intros.
-    injection H ; clear H ; intros H _ ; rewrite -H ; clear H new_scope1.
-    injection H0 ; clear H0 ; intros H0 _ _ ; rewrite -H0 ; clear H0 new_scope2.
-    by exact H1.
-  + simpl stmts_tmap ; simpl ExpandBranch_funs ; simpl stmts_have_fully_inferred_ground_types ; intros.
-    move /andP : H2 => [H2 H3].
-    specialize (ExpandBranch_stmt_tmap vm h old_tmap)
-          with (old_scope1 := old_scope1) (old_scope2 := old_scope2)
-               (old_def_ss := old_def_ss) (old_conn_map := old_conn_map).
-    destruct (stmt_tmap (old_tmap, old_scope1) h vm) as [[tmap' scope']|] ; last by discriminate H.
-    specialize ExpandBranch_stmt_tmap
-          with (new_tmap := tmap') (new_scope1 := scope').
-    destruct (ExpandBranch_fun h old_def_ss old_conn_map old_scope2) as [[[temp_def_ss temp_conn_map] temp_scope]|]; last by discriminate H0.
-    specialize (ExpandBranch_stmt_tmap temp_scope temp_def_ss temp_conn_map Logic.eq_refl Logic.eq_refl H1 H2).
-    by apply (IHss tmap' new_tmap scope' new_scope1 temp_scope new_scope2
-                temp_def_ss new_def_ss temp_conn_map new_conn_map H H0
-                ExpandBranch_stmt_tmap H3).
-Qed.
-*)
-
-Lemma ExpandBranch_stmt_tmap :
-forall (vm : CEP.t vertex_type) (s : HiFP.hfstmt)
-       (old_tmap new_tmap old_scope1 new_scope1 old_scope2 new_scope2 : CEP.t ftype)
-       (old_def_ss new_def_ss : HiFP.hfstmt_seq) (old_conn_map new_conn_map : CEP.t def_expr),
-   stmt_tmap (old_tmap, old_scope1) s vm = Some (new_tmap, new_scope1) ->
-   ExpandBranch_fun s old_def_ss old_conn_map old_scope2 = Some (new_def_ss, new_conn_map, new_scope2) ->
-   submap old_scope2 old_scope1 ->
-   stmt_has_fully_inferred_ground_types s ->
-      submap new_scope2 new_scope1
-with ExpandBranch_stmts_tmap :
-forall (vm : CEP.t vertex_type) (ss : HiFP.hfstmt_seq)
-       (old_tmap new_tmap old_scope1 new_scope1 old_scope2 new_scope2 : CEP.t ftype)
-       (old_def_ss new_def_ss : HiFP.hfstmt_seq) (old_conn_map new_conn_map : CEP.t def_expr),
-   stmts_tmap (old_tmap, old_scope1) ss vm = Some (new_tmap, new_scope1) ->
-   ExpandBranch_funs ss old_def_ss old_conn_map old_scope2 = Some (new_def_ss, new_conn_map, new_scope2) ->
-   submap old_scope2 old_scope1 ->
-   stmts_have_fully_inferred_ground_types ss ->
-      submap new_scope2 new_scope1.
+      CEP.submap new_scope2 new_scope1.
 Proof.
 * clear ExpandBranch_stmt_tmap.
   destruct s ; simpl stmt_tmap ; simpl ExpandBranch_fun ; simpl stmt_has_fully_inferred_ground_types ; intros.
@@ -895,7 +1225,7 @@ Proof.
     destruct (ExpandBranch_funs ss_true old_def_ss old_conn_map old_scope2) as [[[true_def_ss true_conn_map] true_scope2]|] ; last by discriminate H0.
     destruct (stmts_tmap (tmap_true, old_scope1) ss_false vm) as [[tmap_false scope1_false]|] ; last by discriminate H.
     injection H ; clear H ; intros H _ ; rewrite -H ; clear H new_scope1.
-    destruct (ExpandBranch_funs ss_false true_def_ss old_conn_map old_scope2) as [[[false_def_ss false_conn_map] false_scope2]|] ; last by discriminate H0.
+    destruct (ExpandBranch_funs ss_false true_def_ss (extend_map_with old_conn_map true_conn_map) old_scope2) as [[[false_def_ss false_conn_map] false_scope2]|] ; last by discriminate H0.
     injection H0 ; clear H0 ; intros H0 _ _ ; rewrite -H0 ; clear H0 new_scope2.
     by exact H1.
 * clear ExpandBranch_stmts_tmap.
@@ -919,96 +1249,31 @@ Proof.
                 ExpandBranch_stmt_tmap H3).
 Qed.
 
-(*
-The following lemma is probably not needed.
-Lemma ExpandBranch_funs_submap :
-forall (ss : HiFP.hfstmt_seq) (old_def_ss : HiFP.hfstmt_seq) (old_conn_map : CEP.t def_expr) (old_scope : CEP.t ftype),
-   forall (tmap : CEP.t ftype) (vm : CEP.t vertex_type),
-      submap old_scope tmap ->
-      stmts_tmap (tmap, old_scope) ss vm <> None ->
-         match ExpandBranch_funs ss old_def_ss old_conn_map old_scope with
-         | Some (_, _, new_scope) => submap old_scope new_scope
-         | None => True
-         end
-with ExpandBranch_fun_submap :
-forall (s : HiFP.hfstmt) (old_def_ss : HiFP.hfstmt_seq) (old_conn_map : CEP.t def_expr) (old_scope : CEP.t ftype),
-   forall (tmap : CEP.t ftype) (vm : CEP.t vertex_type),
-      submap old_scope tmap ->
-      stmt_tmap (tmap, old_scope) s vm <> None ->
-         match ExpandBranch_fun s old_def_ss old_conn_map old_scope with
-         | Some (_, _, new_scope) => submap old_scope new_scope
-         | None => True
-         end.
-Proof.
-* clear ExpandBranch_funs_submap.
-  induction ss.
-  + intros.
-    unfold ExpandBranch_funs.
-    by apply submap_refl.
-  + intros.
-    simpl stmts_tmap in H0.
-    simpl ExpandBranch_funs.
-    specialize (ExpandBranch_fun_submap h old_def_ss old_conn_map old_scope tmap vm H).
-
-
-
-
-    destruct (stmt_tmap (tmap, old_scope) h vm) as [[tmap' scope']|] ; last by contradiction H0.
-    destruct (ExpandBranch_fun h old_def_ss old_conn_map old_scope) as [[[temp_def_ss temp_conn_map] temp_scope]|] ; last by trivial.
-    specialize (IHss temp_def_ss temp_conn_map temp_scope tmap' vm).
-    destruct (ExpandBranch_funs ss temp_def_ss temp_conn_map temp_scope) as [[[new_def_ss new_conn_map] new_scope]|] ; last by trivial.
-    apply (submap_trans temp_scope).
-    - apply ExpandBranch_fun_submap.
-      discriminate.
-    - apply IHss.
-      (* submap temp_scope tmap' *)
-      (* We now need: submap scope' temp_scope *)
-
-* clear ExpandBranch_fun_submap.
-  intros.
-  destruct H as [vm_old [ct_old [vm_new [ct_new [tmap Hs]]]]].
-  destruct s ; simpl ; simpl in Hs ; try trivial.
-  * (* Sskip *)
-    by apply submap_refl.
-  * (* Swire *)
-    intro.
-
-
-   stmts_have_fully_inferred_ground_types ss ->
-   tmap_has_fully_inferred_ground_types tmap ->
-   submap scope1 tmap ->
-   submap scope2 tmap ->
-   submap scope1 scope2 ->
-      stmts_tmap (tmap, scope1) ss vm = None ->
-         stmts_tmap (tmap, scope2) (component_stmts_of ss) vm <> None ->
-            forall (old_def_ss : HiFP.hfstmt_seq) (old_conn_map : CEP.t def_expr) (old_scope : CEP.t ftype),
-               submap old_scope scope1 ->
-                  ExpandBranch_funs ss old_def_ss old_conn_map old_scope = None
-*)
-
 Lemma ExpandBranch_funs_checks_scopes :
+(* If ss contains a scoping error, then ExpandBranch_funs does not make it go away:
+   either it produces no result, or it produces a result that also contains a scoping error. *)
 forall (ss : HiFP.hfstmt_seq) (tmap scope1 scope2 : CEP.t ftype) (vm : CEP.t vertex_type),
    stmts_have_fully_inferred_ground_types ss ->
    tmap_has_fully_inferred_ground_types tmap ->
-   submap scope1 tmap ->
-   submap scope2 tmap ->
-   submap scope1 scope2 ->
+   CEP.submap scope1 tmap ->
+   CEP.submap scope2 tmap ->
+   CEP.submap scope1 scope2 ->
       stmts_tmap (tmap, scope1) ss vm = None ->
          stmts_tmap (tmap, scope2) (component_stmts_of ss) vm <> None ->
             forall (old_def_ss : HiFP.hfstmt_seq) (old_conn_map : CEP.t def_expr) (old_scope : CEP.t ftype),
-               submap old_scope scope1 ->
+               CEP.submap old_scope scope1 ->
                   ExpandBranch_funs ss old_def_ss old_conn_map old_scope = None
 with ExpandBranch_fun_checks_scopes :
 forall (s : HiFP.hfstmt) (tmap scope1 scope2 : CEP.t ftype) (vm : CEP.t vertex_type),
    stmt_has_fully_inferred_ground_types s ->
    tmap_has_fully_inferred_ground_types tmap ->
-   submap scope1 tmap ->
-   submap scope2 tmap ->
-   submap scope1 scope2 ->
+   CEP.submap scope1 tmap ->
+   CEP.submap scope2 tmap ->
+   CEP.submap scope1 scope2 ->
       stmt_tmap (tmap, scope1) s vm = None ->
          stmts_tmap (tmap, scope2) (component_stmt_of s) vm <> None ->
             forall (old_def_ss : HiFP.hfstmt_seq) (old_conn_map : CEP.t def_expr) (old_scope : CEP.t ftype),
-               submap old_scope scope1 ->
+               CEP.submap old_scope scope1 ->
                   ExpandBranch_fun s old_def_ss old_conn_map old_scope = None.
 Proof.
 * clear ExpandBranch_funs_checks_scopes.
@@ -1087,7 +1352,7 @@ Proof.
     - simpl type_of_ref in H4.
       generalize (H6 s) ; intro.
       destruct (CEP.find s old_scope) as [ft_ref|] ; last by reflexivity.
-      rewrite H7 in H4 ; clear H7.
+      rewrite (H7 _ Logic.eq_refl) in H4 ; clear H7.
       generalize (type_of_expr_submap h0 old_scope scope1 H6) ;
             intro.
       destruct (type_of_expr h0 old_scope) as [[ft_expr p]|] ; last by reflexivity.
@@ -1101,13 +1366,13 @@ Proof.
     - simpl type_of_ref in H4.
       specialize (H6 s).
       destruct (CEP.find s old_scope) as [ft_ref|] ; last by reflexivity.
-      rewrite H6 in H4 ; clear H6.
+      rewrite (H6 _ Logic.eq_refl) in H4 ; clear H6.
       by discriminate H4.
     - destruct h ; try done.
       destruct h ; by done.
   + (* Swhen *)
     rename h into cond ; rename h0 into ss_true ; rename h1 into ss_false.
-    move /andP : H => [Ht Hf].
+    move /andP : H => [/andP [_ Ht] Hf].
     generalize (type_of_expr_submap cond old_scope scope1 H6) ;
           intro.
     destruct (type_of_expr cond old_scope) as [[[[[|[|]]| | | | | |]| |] p]|] ; try by reflexivity.
@@ -1139,17 +1404,198 @@ Proof.
       destruct (stmts_tmap (tmap, scope2) (component_stmts_of ss_true) vm) as [[tmap_true' scope2_true]|] ; last by contradiction H.
       destruct H as [H' H] ; rewrite -H' in H5 H9 H10 ; clear H' tmap_true'.
       destruct (ExpandBranch_funs ss_true old_def_ss old_conn_map old_scope) as [[[true_def_ss true_conn_map] _]|] ; last by reflexivity.
-      assert (submap scope1 tmap_true) by (apply (submap_trans scope1_true) ; apply H8).
-      assert (submap scope1 scope2_true) by (apply (submap_trans scope2 _ _ H3), H10).
+      assert (CEP.submap scope1 tmap_true) by apply (CEP.Lemmas.submap_trans (proj2 (proj2 H8))), H8.
+      assert (CEP.submap scope1 scope2_true) by apply (CEP.Lemmas.submap_trans H3), H10.
       specialize (ExpandBranch_funs_checks_scopes ss_false tmap_true scope1 scope2_true vm
                   Hf H7 H11 (proj1 H10) H12)
-            with (old_def_ss := true_def_ss) (old_conn_map := old_conn_map) (old_scope := old_scope).
+            with (old_def_ss := true_def_ss) (old_conn_map := (extend_map_with old_conn_map true_conn_map)) (old_scope := old_scope).
       destruct (stmts_tmap (tmap_true, scope1) ss_false vm) as [[]|] ; first by discriminate H4.
       rewrite (ExpandBranch_funs_checks_scopes Logic.eq_refl H5 H6) //.
     - destruct (stmts_tmap (tmap, scope2) (component_stmts_of ss_true) vm) ; last by contradiction H5.
       specialize (H9 Logic.eq_refl) with (old_def_ss := old_def_ss) (old_conn_map := old_conn_map) (old_scope := old_scope).
       rewrite H9 //.
 Qed.
+
+
+Lemma ExpandBranch_funs_preserves_fully_inferred :
+   forall (ss def_ss : HiFP.hfstmt_seq) (conn_map : CEP.t def_expr) (scope : CEP.t ftype)
+          (def_ss' : HiFP.hfstmt_seq) (conn_map' : CEP.t def_expr) (scope' : CEP.t ftype),
+      tmap_has_fully_inferred_ground_types scope ->
+      stmts_have_fully_inferred_ground_types ss ->
+      ct_has_fully_inferred_ground_types conn_map ->
+      ExpandBranch_funs ss def_ss conn_map scope = Some (def_ss', conn_map', scope') ->
+              tmap_has_fully_inferred_ground_types scope'
+          /\
+              ct_has_fully_inferred_ground_types conn_map'
+with ExpandBranch_fun_preserves_fully_inferred :
+   forall (def_ss' : HiFP.hfstmt_seq) (conn_map' : CEP.t def_expr) (scope : CEP.t ftype)
+          (s : HiFP.hfstmt) (def_ss : HiFP.hfstmt_seq) (conn_map : CEP.t def_expr) (scope' : CEP.t ftype),
+      tmap_has_fully_inferred_ground_types scope ->
+      stmt_has_fully_inferred_ground_types s ->
+      ct_has_fully_inferred_ground_types conn_map ->
+      ExpandBranch_fun s def_ss conn_map scope = Some (def_ss', conn_map', scope') ->
+              tmap_has_fully_inferred_ground_types scope'
+          /\
+              ct_has_fully_inferred_ground_types conn_map'.
+Proof.
+* clear ExpandBranch_funs_preserves_fully_inferred.
+  induction ss.
+  + simpl ; intros.
+    injection H2 ; clear H2 ; intros H2 H3 _.
+    split.
+    - rewrite -H2 ; exact H.
+    - rewrite -H3 ; exact H1.
+  + simpl ; intros.
+    move /andP : H0 => H0.
+    specialize ExpandBranch_fun_preserves_fully_inferred
+          with (s := h) (def_ss := def_ss) (conn_map := conn_map) (scope := scope)
+               (1 := H) (2 := proj1 H0) (3 := H1).
+    destruct (ExpandBranch_fun h def_ss conn_map scope) as [[[temp_def_ss temp_conn_map] temp_scope]|] ; last by discriminate H2.
+    specialize (ExpandBranch_fun_preserves_fully_inferred temp_def_ss temp_conn_map temp_scope Logic.eq_refl).
+    apply IHss with (1 := proj1 ExpandBranch_fun_preserves_fully_inferred)
+                    (2 := proj2 H0)
+                    (3 := proj2 ExpandBranch_fun_preserves_fully_inferred)
+                    (4 := H2).
+* clear ExpandBranch_fun_preserves_fully_inferred.
+  destruct s ; simpl.
+  + (* Sskip *)
+    intros.
+    injection H2 ; clear H2 ; intros H2 H3 _.
+    split.
+    - rewrite -H2 ; exact H.
+    - rewrite -H3 ; exact H1.
+  + (* Swire *)
+    intros.
+    injection H2 ; clear H2 ; intros H2 H3 _.
+    destruct f as [gt| |] ; try by discriminate H0.
+    split.
+    - rewrite -H2.
+      intro ; specialize (H v).
+      destruct (v == s) eqn: Hvs.
+      * by rewrite CEP.Lemmas.find_add_eq //.
+      * by rewrite CEP.Lemmas.find_add_neq // /PVM.SE.eq Hvs //.
+    - rewrite -H3.
+      intro ; specialize (H1 k).
+      destruct (k == s) eqn: Hks.
+      * by rewrite CEP.Lemmas.find_add_eq //.
+      * by rewrite CEP.Lemmas.find_add_neq // /PVM.SE.eq Hks //.
+  + (* Sreg *)
+    intros.
+    destruct (reset h).
+    2: destruct (match type_of_expr h0 scope with
+                 | Some _ =>
+                     match type_of_expr h1 scope with
+                     | Some _ => true
+                     | None => false
+                     end
+                 | None => false
+                 end) ; last by discriminate H2.
+    1,2: destruct (type_of_expr (clock h) scope) ; last by discriminate H2.
+    1,2: destruct (type h) as [gt| |] ; try by discriminate H0.
+    1,2: move /andP : H0 => [_ H0].
+    1,2: injection H2 ; clear H2 ; intros H2 H3 _.
+    1,2: split.
+    - 1,3: rewrite -H2.
+      1,2: intro ; specialize (H v).
+      1,2: destruct (v == s) eqn: Hvs ;
+            try (by rewrite CEP.Lemmas.find_add_eq //).
+      1,2: by rewrite CEP.Lemmas.find_add_neq // /PVM.SE.eq Hvs //.
+    - 1,2: rewrite -H3.
+      1,2: intro ; specialize (H1 k).
+      1,2: destruct (k == s) eqn: Hks ;
+            try (by rewrite CEP.Lemmas.find_add_eq //).
+      1,2: by rewrite CEP.Lemmas.find_add_neq // /PVM.SE.eq Hks //.
+  + (* Smem *)
+    intros ; discriminate H2.
+  + (* Sinst *)
+    intros ; discriminate H2.
+  + (* Snode *)
+    intros.
+    generalize (expr_preserves_fully_inferred scope H h H0) ; intro.
+    destruct (type_of_expr h scope) as [[[gt| |] _]|] ; try by done.
+    injection H2 ; clear H2 ; intros H2 H4 _.
+    split.
+    - rewrite -H2.
+      intro ; specialize (H v).
+      destruct (v == s) eqn: Hvs.
+      * by rewrite CEP.Lemmas.find_add_eq //.
+      * by rewrite CEP.Lemmas.find_add_neq // /PVM.SE.eq Hvs //.
+    - rewrite -H4 ; exact H1.
+  + (* Sfcnct *)
+    intros.
+    unfold ExpandBranch_connect in H2.
+    destruct h ; try (by discriminate H2) ;
+          last by (clear -H2 ;
+                   induction h ; try (by discriminate H2) ;
+                   apply IHh ; rewrite -H2 // ;
+                   destruct h ; done).
+    destruct (CEP.find s scope) ; last by discriminate H2.
+    move /andP : H0 => [_ H0].
+    generalize (expr_preserves_fully_inferred scope H h0 H0) ; intro.
+    destruct (type_of_expr h0 scope) as [[[gt| |] _]|] ; try done.
+    destruct (connect_type_compatible false f (Gtyp gt) false) ; last by discriminate H2.
+    injection H2 ; clear H2 ; intros H2 H4 _.
+    split.
+    - rewrite -H2 ; exact H.
+    - rewrite -H4.
+      intro ; specialize (H1 k).
+      destruct (k == s) eqn: Hks.
+      * by rewrite CEP.Lemmas.find_add_eq //.
+      * by rewrite CEP.Lemmas.find_add_neq // /PVM.SE.eq Hks //.
+  + (* Sinvalid *)
+    intros.
+    unfold ExpandBranch_connect in H2.
+    destruct h ; try (by discriminate H2) ;
+          last by (clear -H2 ;
+                   induction h ; try (by discriminate H2) ;
+                   apply IHh ; rewrite -H2 // ;
+                   destruct h ; done).
+    destruct (CEP.find s scope) ; last by discriminate H2.
+    injection H2 ; clear H2 ; intros H2 H3 _.
+    split.
+    - rewrite -H2 ; exact H.
+    - rewrite -H3.
+      intro ; specialize (H1 k).
+      destruct (k == s) eqn: Hks.
+      * by rewrite CEP.Lemmas.find_add_eq //.
+      * by rewrite CEP.Lemmas.find_add_neq // /PVM.SE.eq Hks //.
+  + (* Swhen *)
+    rename h into cond ; rename h0 into ss_true ; rename h1 into ss_false.
+    intros.
+    destruct (type_of_expr cond scope) as [[[[[|[|]]| | | | | |]| |] _]|] ; try by discriminate H2.
+    move /andP : H0 => [/andP H3 H0].
+    generalize (ExpandBranch_funs_preserves_fully_inferred ss_true def_ss conn_map scope) ; intro.
+    destruct (ExpandBranch_funs ss_true def_ss conn_map scope) as [[[true_def_ss true_conn_map] true_scope]|] ;
+          last by discriminate H2.
+    specialize (H4 true_def_ss true_conn_map true_scope H (proj2 H3) H1 Logic.eq_refl).
+    specialize (ExpandBranch_funs_preserves_fully_inferred ss_false true_def_ss (extend_map_with conn_map true_conn_map) scope).
+    destruct (ExpandBranch_funs ss_false true_def_ss
+                            (extend_map_with conn_map true_conn_map)
+                            scope) as [[[false_def_ss false_conn_map] false_scope]|] ;
+          last by discriminate H2.
+    injection H2 ; clear H2 ; intros H2 H5 _.
+    split.
+    - rewrite -H2 ; exact H.
+    - rewrite -H5.
+      intro.
+      rewrite CEP.Lemmas.map2_1bis //.
+      destruct H4 as [_ H4].
+      assert (ct_has_fully_inferred_ground_types (extend_map_with conn_map true_conn_map)).
+            intro.
+            rewrite /extend_map_with CEP.Lemmas.map2_1bis //.
+            specialize (H1 k0).
+            destruct (CEP.find k0 conn_map) as [|] ; done.
+      specialize (ExpandBranch_funs_preserves_fully_inferred false_def_ss false_conn_map false_scope
+                  H H0 H6 Logic.eq_refl).
+      destruct ExpandBranch_funs_preserves_fully_inferred as [_ H7].
+      specialize (H4 k) ; specialize (H7 k).
+      destruct (CEP.find k true_conn_map) as [[| |true_expr]|], (CEP.find k false_conn_map) as [[| |false_expr]|] ; try done.
+      simpl.
+      destruct (true_expr == false_expr) ; first by exact H4.
+      simpl.
+      rewrite (proj1 H3) H4 H7 //.
+Qed.
+
 
 Fixpoint ExpandPort_fun (pp : seq HiFP.hfport) : option (CEP.t def_expr * CEP.t ftype) :=
 (* create a map of def_expr for the port sequence pp.
@@ -1209,11 +1655,11 @@ Qed.
 
 Lemma ExpandPort_Sem :
 (* Sem_frag_ports and ExpandPort_fun produce essentially the same port map *)
-forall (tmap : CEP.t ftype) (pp : seq HiFP.hfport) (vm : CEP.t vertex_type) (ct : CEP.t def_expr),
+forall (tmap : CEP.t ftype) (pp : seq HiFP.hfport) (vm vm_tmap : CEP.t vertex_type) (ct : CEP.t def_expr),
     ports_have_fully_inferred_ground_types pp ->
-    match ports_tmap pp vm with
+    match ports_tmap pp vm_tmap with
     | Some pmap =>
-        submap pmap tmap ->
+        CEP.submap pmap tmap ->
         Sem_frag_ports (CEP.empty vertex_type) (CEP.empty def_expr) pp vm ct tmap ->
            match ExpandPort_fun pp with
            | Some (new_conn_map, new_scope) =>
@@ -1225,15 +1671,15 @@ forall (tmap : CEP.t ftype) (pp : seq HiFP.hfport) (vm : CEP.t vertex_type) (ct 
 Proof.
 induction pp ; first by (simpl ; intros ; destruct H1 ; rewrite H2 ; reflexivity).
 intros.
-generalize (ports_tmap_preserves_fully_inferred vm (a :: pp) H) ; intro.
+generalize (ports_tmap_preserves_fully_inferred vm_tmap (a :: pp) H) ; intro.
 simpl ports_have_fully_inferred_ground_types in H.
-generalize (ports_tmap_names vm pp) ; intro.
-generalize (ports_tmap_uniq vm (a :: pp)) ; intro.
-destruct (ports_tmap (a :: pp) vm) as [pmap|] eqn: Hpmap ; last by trivial.
+generalize (ports_tmap_names vm_tmap pp) ; intro.
+generalize (ports_tmap_uniq vm_tmap (a :: pp)) ; intro.
+destruct (ports_tmap (a :: pp) vm_tmap) as [pmap|] eqn: Hpmap ; last by trivial.
 intros.
 simpl ports_tmap in Hpmap.
 destruct H4 as [vm' [ct' [H4 H5]]].
-assert (submap vm' vm /\ submap ct' ct)
+assert (CEP.submap vm' vm /\ CEP.submap ct' ct)
       by (apply Sem_frag_ports_submap with (pp := [:: a]) (tmap := tmap) ;
           simpl ; exists vm', ct' ;
           split ; last (by exact H5) ; split ; reflexivity).
@@ -1242,14 +1688,14 @@ destruct (ExpandPort_fun (a :: pp)) as [[new_conn_map new_scope]|] eqn: Hexpand 
 simpl ExpandPort_fun in Hexpand.
 destruct a as [p [gt| |]|p [gt| |]] ; try done.
 1,2: move /andP : H => [H H7].
-1,2: specialize (IHpp vm' ct' H7).
+1,2: specialize (IHpp vm' vm_tmap ct' H7).
 1,2: destruct (ExpandPort_fun pp) as [[temp_conn_map temp_scope]|] ; last by discriminate Hexpand.
 1,2: injection Hexpand ; clear Hexpand ; intros _ Hexpand ;
      rewrite -Hexpand ; clear new_conn_map new_scope temp_scope Hexpand.
-1,2: generalize (fully_inferred_does_not_change gt p vm H) ; intro.
-1,2: destruct (code_type_find_vm_widths (Gtyp gt) p vm) as [[[gt'| |] _]|] ; try by done.
+1,2: generalize (fully_inferred_does_not_change gt p vm_tmap H) ; intro.
+1,2: destruct (code_type_find_vm_widths (Gtyp gt) p vm_tmap) as [[[gt'| |] _]|] ; try by done.
 1,2: rewrite -H8 in Hpmap ; clear gt' H8.
-1,2: destruct (ports_tmap pp vm) as [pmap'|] eqn: Hports_tmap ; last by done.
+1,2: destruct (ports_tmap pp vm_tmap) as [pmap'|] eqn: Hports_tmap ; last by done.
 1,2: specialize (H1 p).
 1,2: destruct (CEP.find p pmap') eqn: Hfindp' ; first by done.
 1,2: destruct H1 as [H1 _].
@@ -1257,164 +1703,65 @@ destruct a as [p [gt| |]|p [gt| |]] ; try done.
 1,2: rewrite -Hpmap in H0, H3 ; clear pmap Hpmap.
 1,2: generalize (H3 p) ; intro.
 1,2: rewrite CEP.Lemmas.find_add_eq in H8 ; last by rewrite /CEP.SE.eq //.
-1,2: rewrite H8 in H5.
-1,2: simpl size_of_ftype in H5 ; simpl list_rhs_type_p in H5.
-(* First goal: we use proj2 (proj2 H5) and IHpp to prove the result.
-   We only need to prove that ports_tmap pp vm' is Some pmap and is a submap of tmap;
-   that should be possible to prove by using the other parts of H5,
-   which state that vm and vm' are almost the same, so we finally get
-   ports_tmap pp vm is basically CEP.Equal to ports_tmap pp vm'. *)
-* destruct H5 as [_ [H9 H10]].
-  (*specialize (H5 0) ; rewrite /List.nth_error add0n nat_of_binK -surjective_pairing in H5.*)
-  intro.
-  specialize (H10 y).
-  rewrite -H10 ; destruct H6 as [H6 _] ; clear ct H10.
-  assert (ports_tmap pp vm' = ports_tmap pp vm).
-        clear -H2 H7 H9.
-        revert H2 H7.
-        induction pp ;
-              first by (unfold ports_tmap ; reflexivity).
-        intros ; simpl ports_tmap.
-        simpl ports_have_fully_inferred_ground_types in H7.
-        destruct a as [p0 [gt0| |]|p0 [gt0| |]] ; try done.
-        1,2: simpl uniq in H2 ; move /andP : H2 => [H21 /andP [_ H23]].
-        1,2: rewrite in_cons negb_or in H21.
-        1,2: move /andP : H21 => [H21 H22].
-        1,2: move /andP : H7 => [H H7].
-        1,2: simpl uniq in IHpp.
-        1,2: rewrite H22 H23 andTb in IHpp.
-        1,2: specialize (IHpp is_true_true H7).
-        1,2: rewrite IHpp.
-        1,2: assert (CEP.find p0 vm' = CEP.find p0 vm)
-              by (specialize (H9 p0.1 p0.2) ;
-                  rewrite add1n -surjective_pairing in H9 ;
-                  specialize (N.eq_dec p0.1 p.1) ; intro ;
-                  destruct H0 ; last (by apply H9 ; left ; exact n) ;
-                  destruct (Nat.compare_spec p0.2 p.2) ;
-                        first (by specialize (injective_projections p0 p e) ; intro ;
-                                  rewrite -(nat_of_binK p0.2) -(nat_of_binK p.2) H0 in H1 ;
-                                  specialize (H1 Logic.eq_refl) ;
-                                  rewrite H1 eq_refl // in H21) ;
-                        first (by apply H9 ; right ; left  ; move /ltP : H0 => H0 ; exact H0) ;
-                  apply H9 ; right ; right ; move /ltP : H0 => H0 ; exact H0).
-        1,2: unfold code_type_find_vm_widths ;
-             rewrite H0 ;
-             fold (code_type_find_vm_widths (Gtyp gt0) p0 vm).
-        1,2: reflexivity.
-  rewrite H5 Hports_tmap in IHpp.
-  apply IHpp ; last by exact H4.
-  intro.
-  specialize (H3 v).
-  destruct (v == p) eqn: Hvp ; first by move /eqP : Hvp => Hvp ; rewrite Hvp Hfindp' //.
-  rewrite CEP.Lemmas.find_add_neq // in H3.
-  rewrite /PVM.SE.eq Hvp //.
-(* Second goal: similar, just that an element is added to ct. *)
-* destruct H5 as [_ [H9 [H10 H11]]].
-  (*specialize (H5 0) ; rewrite /List.nth_error add0n nat_of_binK -surjective_pairing in H5.*)
-  intro.
-  specialize (H10 y.1 y.2) ; rewrite add1n -surjective_pairing in H10.
-  specialize (H11 0 is_true_true) ; rewrite add0n nat_of_binK -surjective_pairing in H11.
-  destruct (y == p) eqn: Hyp ;
-        first by (move /eqP : Hyp => Hyp ;
-                  rewrite CEP.Lemmas.find_add_eq /PVM.SE.eq Hyp // ;
-                  apply H11).
-  clear H11.
-  rewrite CEP.Lemmas.find_add_neq ; last by rewrite /PVM.SE.eq Hyp //.
-  assert (CEP.find y ct' = CEP.find y ct)
-        by (specialize (N.eq_dec y.1 p.1) ; intro ;
-            destruct H5 ; last (by apply H10 ; left ; exact n) ;
-            destruct (Nat.compare_spec y.2 p.2) ;
-                        first (by specialize (injective_projections y p e) ; intro ;
-                                  rewrite -(nat_of_binK y.2) -(nat_of_binK p.2) H5 in H11 ;
-                                  specialize (H11 Logic.eq_refl) ;
-                                  rewrite H11 eq_refl // in Hyp) ;
-                        first (by apply H10 ; right ; left  ; move /ltP : H5 => H5 ; exact H5) ;
-                  apply H10 ; right ; right ; move /ltP : H5 => H5 ; exact H5).
-  rewrite -H5 ; destruct H6 as [H6 _] ; clear ct H5 H10.
-  assert (ports_tmap pp vm' = ports_tmap pp vm).
-        clear -H2 H7 H9.
-        revert H2 H7.
-        induction pp ;
-              first by (unfold ports_tmap ; reflexivity).
-        intros ; simpl ports_tmap.
-        simpl ports_have_fully_inferred_ground_types in H7.
-        destruct a as [p0 [gt0| |]|p0 [gt0| |]] ; try done.
-        1,2: simpl uniq in H2 ; move /andP : H2 => [H21 /andP [_ H23]].
-        1,2: rewrite in_cons negb_or in H21.
-        1,2: move /andP : H21 => [H21 H22].
-        1,2: move /andP : H7 => [H H7].
-        1,2: simpl uniq in IHpp.
-        1,2: rewrite H22 H23 andTb in IHpp.
-        1,2: specialize (IHpp is_true_true H7).
-        1,2: rewrite IHpp.
-        1,2: assert (CEP.find p0 vm' = CEP.find p0 vm)
-              by (specialize (H9 p0.1 p0.2) ;
-                  rewrite add1n -surjective_pairing in H9 ;
-                  specialize (N.eq_dec p0.1 p.1) ; intro ;
-                  destruct H0 ; last (by apply H9 ; left ; exact n) ;
-                  destruct (Nat.compare_spec p0.2 p.2) ;
-                        first (by specialize (injective_projections p0 p e) ; intro ;
-                                  rewrite -(nat_of_binK p0.2) -(nat_of_binK p.2) H0 in H1 ;
-                                  specialize (H1 Logic.eq_refl) ;
-                                  rewrite H1 eq_refl // in H21) ;
-                        first (by apply H9 ; right ; left  ; move /ltP : H0 => H0 ; exact H0) ;
-                  apply H9 ; right ; right ; move /ltP : H0 => H0 ; exact H0).
-        1,2: unfold code_type_find_vm_widths ;
-             rewrite H0 ;
-             fold (code_type_find_vm_widths (Gtyp gt0) p0 vm).
-        1,2: reflexivity.
-  rewrite H5 Hports_tmap in IHpp.
-  apply IHpp ; last by exact H4.
-  intro.
-  specialize (H3 v).
-  destruct (v == p) eqn: Hvp ; first by move /eqP : Hvp => Hvp ; rewrite Hvp Hfindp' //.
-  rewrite CEP.Lemmas.find_add_neq // in H3.
-  rewrite /PVM.SE.eq Hvp //.
+1,2: rewrite (H8 _ Logic.eq_refl) in H5.
+1,2: simpl size_of_ftype in H5.
+1,2: intro.
+1,2: specialize (IHpp (CEP.Lemmas.submap_add_find_none H3 Hfindp') H4).
+1,2: destruct (y.1 != p.1) eqn: Hyp1 ; move /eqP : Hyp1 => Hyp1.
+* 1,3: destruct H5 as [_ H5] ; specialize (H5 y.1 y.2 (or_introl Hyp1)).
+  1,2: rewrite -surjective_pairing in H5 ; rewrite -(proj2 H5).
+  2: rewrite CEP.Lemmas.find_add_neq ; last by contradict Hyp1 ; move /eqP : Hyp1 => Hyp1 ; rewrite Hyp1 //.
+  1,2: by apply IHpp.
+* 1,2: destruct (y.2 < p.2) eqn: Hypsmall.
+  + 1,3: destruct H5 as [_ H5] ; specialize (H5 y.1 y.2 (or_intror (or_introl Hypsmall))).
+    1,2: rewrite -surjective_pairing in H5 ; rewrite -(proj2 H5).
+    2: rewrite CEP.Lemmas.find_add_neq ;
+          last by (rewrite ltnNge in Hypsmall ; move /negP : Hypsmall => Hypsmall ;
+                   contradict Hypsmall ; move /eqP : Hypsmall => Hypsmall ;
+                   rewrite Hypsmall leqnn //).
+    1,2: by apply IHpp.
+  + 1,2: rewrite add1n in H5.
+    1,2: destruct (p.2 < y.2) eqn: Hyplarge.
+    - 1,3: destruct H5 as [_ H5] ; specialize (H5 y.1 y.2 (or_intror (or_intror Hyplarge))).
+      1,2: rewrite -surjective_pairing in H5 ; rewrite -(proj2 H5).
+      2: rewrite CEP.Lemmas.find_add_neq ;
+            last by (rewrite ltnNge in Hyplarge ; move /negP : Hyplarge => Hyplarge ;
+                     contradict Hyplarge ; move /eqP : Hyplarge => Hyplarge ;
+                     rewrite Hyplarge leqnn //).
+      1,2: by apply IHpp.
+    - 1,2: destruct H5 as [H5 _] ; simpl in H5.
+      1,2: move /and3P : H5 => [_ H5 H9].
+      1,2: apply negbT in Hypsmall ; rewrite -leqNgt in Hypsmall.
+      1,2: apply negbT in Hyplarge ; rewrite -leqNgt in Hyplarge.
+      1,2: assert (nat_of_bin y.2 == nat_of_bin p.2)
+            by (rewrite eqn_leq Hypsmall Hyplarge //).
+      1,2: move /eqP : H10 => H10.
+      1,2: assert (y = p)
+            by (apply injective_projections ;
+                first (by apply Hyp1) ;
+                last (by rewrite -(nat_of_binK y.2) H10 nat_of_binK //)).
+      1,2: move /eqP : H5 => H5 ; move /eqP : H9 => H9.
+      1,2: rewrite H11 H9 -IHpp.
+      * rewrite H5 //.
+      * rewrite CEP.Lemmas.find_add_eq // /PVM.SE.eq //.
 Qed.
 
-(*
-Theorem ExpandBranch_Sem :
-forall (vm : CEP.t vertex_type) (pp : seq HiFP.hfport) (ss : HiFP.hfstmt_seq),
-    ports_have_fully_inferred_ground_types pp ->
-    stmts_have_fully_inferred_ground_types ss ->
-    match port_stmts_tmap pp ss vm with
-    | Some tmap =>
-        match ExpandPort_fun pp with
-        | Some (port_conn_map, _) =>
-            match ExpandBranch_funs ss (Qnil ProdVarOrder.T) port_conn_map tmap with
-            | Some (def_ss, conn_map) =>
-                exists (vm' vm_new : CEP.t ftype),
-                              Sem_frag_ports (CEP.empty vertex_type) (CEP.empty def_expr) pp vm' port_conn_map tmap
-                           /\ Sem_frag_stmts vm' port_conn_map ss vm_new conn_map
-                        (* /\ vm_new is the extension of vm' with def_ss *)
-            | None => True
-            end
-        | None => True
-        end
-    | None => True
-    end.
-*)
 
-Definition helper_connect (v : ProdVarOrder.t) (d : def_expr) (old_ss : option HiFP.hfstmt_seq) : option HiFP.hfstmt_seq :=
-(* The helper function adds a connect statement for reference v *)
-match old_ss, d with
-| None, _ (* propagate earlier error *)
-| _, D_undefined => None (* component v is still not connected; error *)
-| Some old_ss, D_invalidated => Some (Qrcons old_ss (Sinvalid (Eid v)))
-| Some old_ss, D_fexpr e => Some (Qrcons old_ss (Sfcnct (Eid v) e))
+Definition helper_connect (v : ProdVarOrder.t) (d : def_expr) (old_ss : HiFP.hfstmt_seq) : HiFP.hfstmt_seq :=
+(* The helper function adds a connect statement for reference v.
+   If the value is undefined, then silently nothing will be changed. *)
+match d with
+| D_undefined => old_ss (* component v is still not connected; error *)
+| D_invalidated => Qcons (Sinvalid (Eid v)) old_ss
+| D_fexpr e => Qcons (Sfcnct (Eid v) e) old_ss
 end.
 
 Lemma fold_connect_components :
-forall conn_map : CEP.t def_expr,
-      CEP.fold helper_connect conn_map None = None
-   /\
-      forall ss : HiFP.hfstmt_seq,
-         match CEP.fold helper_connect conn_map (Some ss) with
-         | Some conn_ss => component_stmts_of conn_ss = component_stmts_of ss
-         | None => True
-         end.
+forall (conn_map : CEP.t def_expr) (ss : HiFP.hfstmt_seq),
+    component_stmts_of (CEP.fold helper_connect conn_map ss) = component_stmts_of ss.
 Proof.
 intro.
+(*
 assert (forall l : list (CEP.key * def_expr),
           List.fold_left
              (fun (a : option HiFP.hfstmt_seq) (p : CEP.key * def_expr)
@@ -1422,7 +1769,7 @@ assert (forall l : list (CEP.key * def_expr),
       induction l.
       * unfold List.fold_left ; by reflexivity.
       * simpl List.fold_left ; apply IHl.
-split ; first by rewrite CEP.fold_1 ; apply H.
+split ; first by rewrite CEP.fold_1 ; apply H. *)
 intros.
 rewrite CEP.fold_1.
 revert ss.
@@ -1430,32 +1777,468 @@ generalize (CEP.elements conn_map).
 induction l.
 * intro ; simpl ; by reflexivity.
 * intro ; simpl List.fold_left.
-  destruct a.2 ; try (rewrite H ; trivial).
-  + assert (component_stmts_of ss = component_stmts_of (Qrcons ss (Sinvalid (Eid (var:=ProdVarOrder.T) a.1)))).
-          induction ss.
-          + simpl ; by reflexivity.
-          + simpl ; rewrite IHss ; by reflexivity.
-    rewrite H0.
-    apply IHl.
-  + assert (component_stmts_of ss = component_stmts_of (Qrcons ss (Sfcnct (Eid (var:=ProdVarOrder.T) a.1) h))).
-          induction ss.
-          + simpl ; by reflexivity.
-          + simpl ; rewrite IHss ; by reflexivity.
-    rewrite H0.
-    apply IHl.
+  destruct a as [k []] ; simpl ; rewrite IHl //.
 Qed.
 
-Theorem ExpandBranches_Sem :
+Definition extend_defined_map_with (m dflt : CEP.t def_expr) : CEP.t def_expr :=
+(* Returns map m, except that undefined elements are copied from dflt.
+   “undefined” here includes expressions that are assigned an undefined value *)
+CEP.map2 (fun (elm eld : option def_expr) => match elm with
+                                      | Some D_undefined | None => eld
+                                      | _ => elm
+                                      end) m dflt.
+
+(*
+Lemma test : forall (k : CEP.key) (v : def_expr), CEP.eq_key_elt (k,v) (k,v).
+Proof.
+rewrite /CEP.eq_key_elt /CEP.SE.eq.
+split.
+- apply eq_refl.
+- reflexivity.
+Qed.
+
+Print test.
+*)
+
+
+(* a lemma that states that helper_connect and Sem_frag_stmts are sort of inverses *)
+Lemma helper_connect_Sem :
+forall (conn_map : CEP.t def_expr) (vm_old : CEP.t vertex_type) (ct_old : CEP.t def_expr) (vm_new : CEP.t vertex_type) (ct_new : CEP.t def_expr) (tmap: CEP.t ftype),
+    tmap_has_fully_inferred_ground_types tmap ->
+    ct_has_fully_inferred_ground_types conn_map ->
+            (Sem_frag_stmts vm_old ct_old (CEP.fold helper_connect conn_map (Qnil ProdVarOrder.T)) vm_new ct_new tmap ->
+                    CEP.Equal vm_old vm_new
+                /\
+                    CEP.Equal ct_new (extend_defined_map_with conn_map ct_old))
+        (*/\
+            (vm_and_ct_compatible vm_old ct_old ->
+            CEP.submap conn_map ct_old ->
+            CEP.Equal vm_old vm_new ->
+            CEP.Equal ct_new (extend_defined_map_with conn_map ct_old) ->
+            "type correctness according to tmap" ->
+            (* or perhaps write something like a weak semantics, i.e.
+               "if there is no error, then ..." *)
+                Sem_frag_stmts vm_old ct_old (CEP.fold helper_connect conn_map (Qnil ProdVarOrder.T)) vm_new ct_new tmap)*).
+Proof.
+intros until 2.
+(*split.*)
+* rewrite CEP.Lemmas.P.fold_spec_right.
+  assert (SetoidList.equivlistA (PVM.eq_key_elt (elt:=def_expr))
+                                (List.rev (CEP.elements conn_map))
+                                (CEP.elements conn_map))
+        by (intro ;
+            apply (SetoidList.InA_rev (PVM.eq_key_elt (elt:=def_expr)))).
+  revert H1.
+  generalize (CEP.elements_3w conn_map) ; intro.
+  assert (Heqv_key : RelationClasses.Equivalence (CEP.eq_key (elt:=def_expr))).
+        clear.
+        assert (forall x : CEP.key * def_expr, CEP.eq_key x x)
+              by (intro ; rewrite /CEP.eq_key /CEP.SE.eq eq_refl //).
+        assert (forall x y : CEP.key * def_expr, CEP.eq_key x y -> CEP.eq_key y x)
+              by (intros ; rewrite /CEP.eq_key /CEP.SE.eq eq_sym H0 //).
+        assert (forall x y z : CEP.key * def_expr, CEP.eq_key x y -> CEP.eq_key y z -> CEP.eq_key x z)
+              by (intros ; rewrite H1 H2 /CEP.eq_key /CEP.SE.eq //).
+        exact (RelationClasses.Build_Equivalence (CEP.eq_key (elt:=def_expr)) H H0 H1).
+  assert (Heqv_key_elt : RelationClasses.Equivalence (CEP.eq_key_elt (elt:=def_expr))).
+        clear.
+        assert (forall x : CEP.key * def_expr, CEP.eq_key_elt x x)
+              by (destruct x ; split ; first (by rewrite /CEP.SE.eq eq_refl //) ; last (by reflexivity)).
+        assert (forall x y : CEP.key * def_expr, CEP.eq_key_elt x y -> CEP.eq_key_elt y x)
+              by (destruct x, y ; split ; first (by rewrite /CEP.SE.eq eq_sym (proj1 H0) //) ; last (by symmetry ; apply H0)).
+        assert (forall x y z : CEP.key * def_expr, CEP.eq_key_elt x y -> CEP.eq_key_elt y z -> CEP.eq_key_elt x z)
+              by (destruct x, y, z ; split ; first (by rewrite (proj1 H1) (proj1 H2) /CEP.SE.eq //) ;
+                  last (by apply (eq_trans (proj2 H1) (proj2 H2)))).
+        exact (RelationClasses.Build_Equivalence (CEP.eq_key_elt (elt:=def_expr)) H H0 H1).
+  assert (Heqv_key0 : RelationClasses.Equivalence (fun x y : ProdVarOrder.T => x == y)).
+        clear.
+        assert (forall x y : ProdVarOrder.T, x == y -> y == x)
+              by (intros ; rewrite eq_sym //).
+        assert (forall x y z : ProdVarOrder.T, x == y -> y == z -> x == z)
+              by (intros ; move /eqP : H0 => H0 ; rewrite H0 //).
+        exact (RelationClasses.Build_Equivalence (fun x y : ProdVarOrder.T => x == y) (eq_refl (T := ProdVarOrder.T)) H H0).
+  assert (InA_In : forall (k : CEP.key) (d : def_expr) (conn_map_list : seq (CEP.key * def_expr)),
+              SetoidList.InA (@CEP.eq_key_elt def_expr) (* (fun p p' : PVM.SE.t * def_expr => PVM.SE.eq p.1 p'.1 /\ p.2 = p'.2) *)
+                             (k, d) conn_map_list ->
+                  List.In (k, d) conn_map_list).
+        (* I think this might be some lemma but I cannot find it... *)
+        clear ; intros.
+        induction conn_map_list.
+        + apply SetoidList.InA_nil in H ; contradiction H.
+        + destruct ((k, d) == a) eqn: Hkda ; move /eqP : Hkda => Hkda ;
+                first by (rewrite Hkda ; apply List.in_eq).
+          apply List.in_cons, IHconn_map_list.
+          inversion H ; last by exact H1.
+          clear H0 H2 l y.
+          destruct H1.
+          rewrite /PVM.SE.eq in H0 ; move /eqP : H0 => H0.
+          by generalize (injective_projections (k,d) a H0 H1) ; contradiction.
+  apply SetoidList.NoDupA_rev in H1 ; last by apply Heqv_key.
+  revert H0 H1.
+  generalize (List.rev (CEP.elements conn_map)) as conn_map_list.
+  intro ; revert conn_map_list vm_old ct_old conn_map.
+  induction conn_map_list.
+  + unfold List.fold_right.
+    intros.
+    split ; first by apply H3.
+    intro.
+    apply RelationClasses.Equivalence_Symmetric, SetoidList.equivlistA_nil_eq in H2 ;
+          last by exact Heqv_key_elt.
+    apply CEP.Lemmas.P.elements_Empty in H2.
+    apply CEP.Lemmas.Empty_find with (x := y) in H2.
+    simpl Sem_frag_stmts in H3.
+    unfold extend_map_with.
+    rewrite CEP.Lemmas.map2_1bis // H2.
+    symmetry ; apply H3.
+  + destruct a as [k v].
+    simpl List.fold_right.
+    intros until 3.
+    (*destruct (List.fold_right (CEP.Lemmas.P.uncurry helper_connect)
+                              (Qnil ProdVarOrder.T) conn_map_list) eqn: Hfold ;
+          rewrite Hfold // /CEP.Lemmas.P.uncurry /helper_connect /fst /snd.
+    rewrite Hfold in IHconn_map_list.*)
+    inversion H1 ; clear H3 H4 x l.
+    assert (forall k : CEP.key,
+                match CEP.find k (CEP.Lemmas.P.of_list conn_map_list) with
+                | Some (D_fexpr e) => expr_has_fully_inferred_ground_types e
+                | _ => true
+                end).
+          intro.
+          generalize (CEP.find_2 (m := CEP.Lemmas.P.of_list conn_map_list) (x := k0)) ; intro.
+          destruct (CEP.find k0 (CEP.Lemmas.P.of_list conn_map_list)) as [[]|] ; try done.
+          specialize (H3 (D_fexpr h) Logic.eq_refl).
+          apply (CEP.Lemmas.P.of_list_1 k0 (D_fexpr h) H6), (SetoidList.InA_cons_tl (k, v)),
+                H2, CEP.Lemmas.elements_mapsto_iff, CEP.find_1 in H3.
+          specialize (H0 k0) ; rewrite H3 // in H0.
+    destruct v.
+    - (* D_undefined *)
+      unfold CEP.Lemmas.P.uncurry ; simpl Sem_frag_stmts.
+      intro.
+      specialize (IHconn_map_list vm_old ct_old (CEP.Lemmas.P.of_list conn_map_list)
+                                  H3 H6 (CEP.Lemmas.P.of_list_2 H6) H4).
+      split ; first by apply IHconn_map_list.
+      apply (CEP.Lemmas.Equal_trans (proj2 IHconn_map_list)).
+      intro.
+      unfold extend_map_with.
+      rewrite CEP.Lemmas.map2_1bis // (*CEP.Lemmas.P.of_list_1b //. *)
+              CEP.Lemmas.map2_1bis //.
+      (*
+      specialize (H k).
+      destruct (CEP.find k tmap) as [[gt| |]|] ; try by contradiction.
+      rewrite /size_of_ftype /mkseq in H3 ; simpl in H3.
+      rewrite N.add_0_r -surjective_pairing in H3. *)
+      destruct (y == k) eqn: Hyk.
+      + move /eqP : Hyk => Hyk.
+        rewrite Hyk.
+        destruct (PVM.find k (CEP.Lemmas.P.of_list conn_map_list)) eqn: Hfind_list.
+        - contradict H5.
+          apply (SetoidList.InA_eqA Heqv_key (x := (k, d))) ;
+                first by rewrite /CEP.eq_key /fst /CEP.SE.eq //.
+          apply SetoidList.In_InA ; first by exact Heqv_key.
+          rewrite CEP.Lemmas.P.of_list_1b // in Hfind_list.
+          apply SetoidList.findA_NoDupA in Hfind_list ;
+                last (by exact H6) ;
+                last (by exact Heqv_key0).
+          apply InA_In, Hfind_list.
+        - (* use H2 to show that PVM.find k conn_map = D_undefined *)
+          rewrite (CEP.Lemmas.elements_o conn_map k).
+          generalize (SetoidList.findA_NoDupA Heqv_key0 HiFP.PVSLemmas.P.FM.eq_dec
+                      (l := CEP.elements conn_map) k D_undefined (CEP.elements_3w conn_map)) ; intro.
+          rewrite (proj1 H7) //.
+          apply H2, SetoidList.InA_cons_hd.
+          by done.
+      + destruct (PVM.find y (CEP.Lemmas.P.of_list conn_map_list)) eqn: Hfind_list.
+        - specialize (H2 (y, d)).
+          destruct H2 as [H2 _].
+          rewrite CEP.Lemmas.P.of_list_1b in Hfind_list ; last by apply H6.
+          apply SetoidList.findA_NoDupA in Hfind_list ;
+                last (by apply H6) ; last by apply Heqv_key0.
+          apply SetoidList.InA_cons_tl with (y := (k, D_undefined)) in Hfind_list.
+          apply H2, CEP.elements_2, CEP.find_1 in Hfind_list.
+          rewrite Hfind_list //.
+        - destruct (PVM.find y conn_map) eqn: Hfind_map.
+          * apply CEP.find_2, CEP.elements_1, H2, SetoidList.InA_cons in Hfind_map.
+            destruct Hfind_map as [Hfind_map|Hfind_map] ;
+                  first (by rewrite /PVM.eq_key_elt /PVM.Raw.Proofs.PX.eqke /fst Hyk in Hfind_map ;
+                            destruct Hfind_map as [Hfind_map _] ; done).
+            rewrite CEP.Lemmas.P.of_list_1b in Hfind_list ; last by exact H6.
+            apply (SetoidList.findA_NoDupA Heqv_key0 ProdVarOrder.eq_dec y d H6) in Hfind_map.
+            rewrite Hfind_map // in Hfind_list.
+          * by reflexivity.
+    - (* D_invalidated *)
+      simpl Sem_frag_stmts.
+      intro.
+      destruct H4 as [vm' [ct' [[H4 H7] H8]]].
+      specialize (IHconn_map_list vm' ct' (CEP.Lemmas.P.of_list conn_map_list)
+                                  H3 H6 (CEP.Lemmas.P.of_list_2 H6) H8).
+      split ; first by apply (CEP.Lemmas.Equal_trans H4), IHconn_map_list.
+      apply (CEP.Lemmas.Equal_trans (proj2 IHconn_map_list)).
+      intro.
+      unfold extend_map_with.
+      rewrite CEP.Lemmas.map2_1bis // (*CEP.Lemmas.P.of_list_1b //. *)
+              CEP.Lemmas.map2_1bis //.
+      specialize (H k).
+      destruct (CEP.find k tmap) as [[gt| |]|] ; try by contradiction.
+      rewrite /size_of_ftype /mkseq in H7 ; simpl in H7.
+      rewrite N.add_0_r -surjective_pairing in H7.
+      destruct (y == k) eqn: Hyk.
+      + move /eqP : Hyk => Hyk.
+        rewrite Hyk.
+        destruct (PVM.find k (CEP.Lemmas.P.of_list conn_map_list)) eqn: Hfind_list.
+        - contradict H5.
+          apply (SetoidList.InA_eqA Heqv_key (x := (k, d))) ;
+                first by rewrite /CEP.eq_key /fst /CEP.SE.eq //.
+          apply SetoidList.In_InA ; first by exact Heqv_key.
+          rewrite CEP.Lemmas.P.of_list_1b // in Hfind_list.
+          apply SetoidList.findA_NoDupA in Hfind_list ;
+                last (by exact H6) ;
+                last (by exact Heqv_key0).
+          apply InA_In, Hfind_list.
+        - (* use H2 to show that PVM.find k conn_map = D_invalidated *)
+          rewrite (CEP.Lemmas.elements_o conn_map k).
+          generalize (SetoidList.findA_NoDupA (B := def_expr) Heqv_key0) ; intro.
+          specialize H9 with (eqA_dec := HiFP.PVSLemmas.P.FM.eq_dec) (l := CEP.elements conn_map) (a := k) (b := D_invalidated) (1 := CEP.elements_3w conn_map).
+          rewrite (proj1 H9).
+          * destruct H7 as [H7 _] ; specialize (H7 0) ; simpl in H7.
+            apply H7.
+          * apply H2, SetoidList.InA_cons_hd.
+            by done.
+      + destruct H7 as [_ H7].
+        specialize (H7 y).
+        rewrite mem_seq1 Hyk in H7.
+        rewrite -H7.
+        destruct (PVM.find y (CEP.Lemmas.P.of_list conn_map_list)) eqn: Hfind_list.
+        - specialize (H2 (y, d)).
+          rewrite CEP.Lemmas.P.of_list_1b in Hfind_list ; last by apply H6.
+          apply SetoidList.findA_NoDupA in Hfind_list ;
+                last (by apply H6) ; last by apply Heqv_key0.
+          apply SetoidList.InA_cons_tl with (y := (k, D_invalidated)) in Hfind_list.
+          apply H2, CEP.elements_2, CEP.find_1 in Hfind_list.
+          rewrite Hfind_list //.
+        - destruct (PVM.find y conn_map) eqn: Hfind_map.
+          * apply CEP.find_2, CEP.elements_1 in Hfind_map.
+            apply H2, SetoidList.InA_cons in Hfind_map.
+            destruct Hfind_map as [Hfind_map|Hfind_map] ;
+                  first (by rewrite /PVM.eq_key_elt /PVM.Raw.Proofs.PX.eqke /fst Hyk in Hfind_map ;
+                            destruct Hfind_map as [Hfind_map _] ; done).
+            rewrite CEP.Lemmas.P.of_list_1b in Hfind_list ; last by exact H6.
+            apply (SetoidList.findA_NoDupA Heqv_key0 ProdVarOrder.eq_dec y d H6) in Hfind_map.
+            rewrite Hfind_map // in Hfind_list.
+          * by reflexivity.
+    - (* Expressions should not be very difficult... *)
+      simpl Sem_frag_stmts.
+      intro.
+      destruct H4 as [vm' [ct' H4]].
+      specialize (H0 k).
+      assert (CEP.eq_key_elt (k, D_fexpr h) (k, D_fexpr h))
+            by (split ; first (by rewrite /CEP.SE.eq //) ; last by reflexivity).
+      apply (SetoidList.InA_cons_hd conn_map_list), H2, CEP.Lemmas.elements_mapsto_iff, CEP.find_1 in H7.
+      rewrite H7 in H0 ; clear H7.
+      destruct h.
+      1-6: destruct H4 as [[H4 H7] H8].
+      1-6: specialize (IHconn_map_list vm' ct' (CEP.Lemmas.P.of_list conn_map_list)
+                                  H3 H6 (CEP.Lemmas.P.of_list_2 H6) H8).
+      1-6: split ; first by apply (CEP.Lemmas.Equal_trans H4), IHconn_map_list.
+      1-6: apply (CEP.Lemmas.Equal_trans (proj2 IHconn_map_list)).
+      1-6: intro.
+      1-6: unfold extend_map_with.
+      1-6: rewrite CEP.Lemmas.map2_1bis // (*CEP.Lemmas.P.of_list_1b //. *)
+              CEP.Lemmas.map2_1bis //.
+      1-6: generalize (H k) ; intro.
+      1-6: destruct (CEP.find k tmap) as [[gt| |]|] ; try by contradiction.
+      1-6: rewrite /size_of_ftype /mkseq in H7 ; simpl in H7.
+      1-6: rewrite N.add_0_r -surjective_pairing in H7.
+      1-6: destruct (y == k) eqn: Hyk.
+      + 1,3,5,7,9,11: move /eqP : Hyk => Hyk.
+        1-6: rewrite Hyk.
+        1-6: destruct (PVM.find k (CEP.Lemmas.P.of_list conn_map_list)) eqn: Hfind_list.
+        - 1,3,5,7,9,11: contradict H5.
+          1-6: apply (SetoidList.InA_eqA Heqv_key (x := (k, d))) ;
+                first by rewrite /CEP.eq_key /fst /CEP.SE.eq //.
+          1-6: apply SetoidList.In_InA ; first by exact Heqv_key.
+          1-6: rewrite CEP.Lemmas.P.of_list_1b // in Hfind_list.
+          1-6: apply SetoidList.findA_NoDupA in Hfind_list ;
+                last (by exact H6) ;
+                last (by exact Heqv_key0).
+          1-6: apply InA_In, Hfind_list.
+        - (* use H1 to show that PVM.find k conn_map = D_invalidated *)
+          1-6: rewrite (CEP.Lemmas.elements_o conn_map k).
+          1-6: generalize (SetoidList.findA_NoDupA (B := def_expr) Heqv_key0) ; intro.
+          1-6: specialize H10 with (eqA_dec := HiFP.PVSLemmas.P.FM.eq_dec) (l := CEP.elements conn_map) (a := k) (1 := CEP.elements_3w conn_map).
+          1: specialize (H10 (D_fexpr (Econst ProdVarOrder.T f b))).
+          2: specialize (H10 (D_fexpr (Ecast u h))).
+          3: specialize (H10 (D_fexpr (Eprim_unop e h))).
+          4: specialize (H10 (D_fexpr (Eprim_binop e h1 h2))).
+          5: specialize (H10 (D_fexpr (Emux h1 h2 h3))).
+          6: specialize (H10 (D_fexpr (Evalidif h1 h2))).
+          1-6: rewrite (proj1 H10) ; last by (apply H2, SetoidList.InA_cons_hd ; done).
+          1: by destruct f, gt ; try (by destruct H7 as [H7 _] ; done) ;
+                destruct H7 as [_ [H7 _]] ; specialize (H7 0) ; simpl in H7 ; apply H7.
+          1: by destruct u, (type_of_expr h tmap) as [[[[| | | | | |]| |] _]|] ; try (by contradiction H7) ;
+                destruct gt ; try (by destruct H7 as [H7 _] ; done) ;
+                destruct H7 as [_ [H7 _]] ; specialize (H7 0) ; simpl in H7 ; apply H7.
+          1: destruct e, (type_of_expr h tmap) as [[[[| | | | | |]| |] _]|] ; try done ;
+             destruct gt ; try (by destruct H7 as [H7 _] ; done) ;
+             try (destruct (n0 <= n < n1)) ;
+             try (destruct (n <= n0)) ; try (by contradiction H7) ;
+             by destruct H7 as [_ [H7 _]] ; specialize (H7 0) ; simpl in H7 ; apply H7.
+          1: by destruct e, (type_of_expr h1 tmap) as [[[[| | | | | |]| |] _]|],
+                            (type_of_expr h2 tmap) as [[[[| | | | | |]| |] _]|] ; try done ;
+                destruct gt ; try (by destruct H7 as [H7 _] ; done) ;
+                destruct H7 as [_ [H7 _]] ; specialize (H7 0) ; simpl in H7 ; apply H7.
+          1: simpl in H0 ; move /andP : H0 => [_ H0] ;
+             generalize (expr_preserves_fully_inferred tmap H h3 H0) ; intro.
+             by destruct (type_of_expr h1 tmap) as [[[[[|[|]]| | | | | |]| |] _]|],
+                         (type_of_expr h2 tmap) as [[[[| | | | | |]| |] p2]|],
+                         (type_of_expr h3 tmap) as [[[[| | | | | |]| |] p3]|] ; try done ;
+                simpl in H7 ;
+                destruct gt ; try (by destruct H7 as [H7 _] ; done) ;
+                destruct H7 as [_ [H7 _]] ; specialize (H7 0) ; simpl in H7 ; apply H7.
+          1: simpl in H0 ; move /andP : H0 => [_ H0] ;
+             generalize (expr_preserves_fully_inferred tmap H h2 H0) ; intro.
+             by destruct (type_of_expr h1 tmap) as [[[[[|[|]]| | | | | |]| |] _]|],
+                         (type_of_expr h2 tmap) as [[[[| | | | | |]| |] _]|] ; try done ;
+                simpl in H7 ;
+                destruct gt ; try (by destruct H7 as [H7 _] ; done) ;
+                destruct H7 as [_ [H7 _]] ; specialize (H7 0) ; simpl in H7 ; apply H7.
+      + 6: simpl in H0 ; move /andP : H0 => [_ H0] ;
+           generalize (expr_preserves_fully_inferred tmap H h2 H0) ; intro ;
+           destruct (type_of_expr h1 tmap) as [[[[[|[|]]| | | | | |]| |] _]|],
+                    (type_of_expr h2 tmap) as [[[[| | | | | |]| |] _]|] ; try done ;
+           destruct gt ; try (by destruct H7 as [H7 _] ; done).
+        5: simpl in H0 ; move /andP : H0 => [_ H0] ;
+           generalize (expr_preserves_fully_inferred tmap H h3 H0) ; intro ;
+           destruct (type_of_expr h1 tmap) as [[[[[|[|]]| | | | | |]| |] _]|],
+                    (type_of_expr h2 tmap) as [[[[| | | | | |]| |] p2]|],
+                    (type_of_expr h3 tmap) as [[[[| | | | | |]| |] p3]|] ; try done ;
+           simpl in H7 ; destruct gt ; try (by destruct H7 as [H7 _] ; done).
+        4: destruct e, (type_of_expr h1 tmap) as [[[[| | | | | |]| |] _]|],
+                       (type_of_expr h2 tmap) as [[[[| | | | | |]| |] _]|] ; try done ;
+                destruct gt ; try (by destruct H7 as [H7 _] ; done).
+        3: destruct e, (type_of_expr h tmap) as [[[[| | | | | |]| |] _]|] ; try done ;
+           destruct gt ; try (by destruct H7 as [H7 _] ; done) ;
+           try (destruct (n0 <= n < n1)) ;
+           try (destruct (n <= n0)) ; try (by contradiction H7).
+        2: destruct u, (type_of_expr h tmap) as [[[[| | | | | |]| |] _]|] ; try (by contradiction H7) ;
+           destruct gt ; try (by destruct H7 as [H7 _] ; done).
+        1: destruct f, gt ; try (by destruct H7 as [H7 _] ; done).
+           1-182: destruct H7 as [_ [_ H7]].
+           1-182: specialize (H7 y).
+           1-182: rewrite mem_seq1 Hyk in H7.
+           1-182: rewrite -H7.
+           1-182: destruct (PVM.find y (CEP.Lemmas.P.of_list conn_map_list)) eqn: Hfind_list ;
+                 try (by specialize (H2 (y, d)) ;
+                         rewrite CEP.Lemmas.P.of_list_1b in Hfind_list ; last (by apply H6) ;
+                         apply SetoidList.findA_NoDupA in Hfind_list ;
+                               last (by apply H6) ; last (by apply Heqv_key0) ;
+                         destruct H2 as [H2 _] ;
+                         apply CEP.elements_2 in H2 ;
+                               last (by apply SetoidList.InA_cons_tl, Hfind_list) ;
+                         rewrite (CEP.find_1 H2) //).
+           1-182: destruct (PVM.find y conn_map) eqn: Hfind_map ;
+                 try (by reflexivity).
+           1-182: apply CEP.find_2, CEP.elements_1 in Hfind_map.
+           1-182: apply H2, SetoidList.InA_cons in Hfind_map.
+           1-182: destruct Hfind_map as [Hfind_map|Hfind_map] ;
+                  try (by rewrite /PVM.eq_key_elt /PVM.Raw.Proofs.PX.eqke /fst Hyk in Hfind_map ;
+                          destruct Hfind_map as [Hfind_map _] ; done).
+           1-182: rewrite CEP.Lemmas.P.of_list_1b in Hfind_list ; try (by exact H6).
+           1-182: apply (SetoidList.findA_NoDupA Heqv_key0 ProdVarOrder.eq_dec y d H6) in Hfind_map.
+           1-182: rewrite Hfind_map // in Hfind_list.
+      (* what remains is a link with a reference, which is translated to a different Sfcnct case. *)
+      destruct H4 as [[H4 H7] H8].
+      specialize (IHconn_map_list vm' ct' (CEP.Lemmas.P.of_list conn_map_list)
+                                  H3 H6 (CEP.Lemmas.P.of_list_2 H6) H8).
+      split ; first by apply (CEP.Lemmas.Equal_trans H4), IHconn_map_list.
+      apply (CEP.Lemmas.Equal_trans (proj2 IHconn_map_list)).
+      intro.
+      unfold extend_map_with.
+      rewrite CEP.Lemmas.map2_1bis // (*CEP.Lemmas.P.of_list_1b //. *)
+              CEP.Lemmas.map2_1bis //.
+      generalize (H k) ; intro.
+      destruct (CEP.find k tmap) as [[gt| |]|] ; try by contradiction.
+      generalize (list_lhs_ref_p_type tmap h) ; intro.
+      destruct (list_lhs_ref_p h tmap) as [[[|ic [|]] [gt_src| |]]|] ; last (by contradiction H7) ;
+            destruct H7 as [_ H7] ; simpl in H7 ; try (by destruct H7 as [H7 _] ; done).
+      rewrite /size_of_ftype /mkseq in H7 ; simpl in H7.
+      rewrite N.add_0_r -surjective_pairing in H7.
+      destruct (y == k) eqn: Hyk.
+      + move /eqP : Hyk => Hyk ; rewrite Hyk.
+        destruct (PVM.find k (CEP.Lemmas.P.of_list conn_map_list)) eqn: Hfind_list.
+        - contradict H5.
+          apply (SetoidList.InA_eqA Heqv_key (x := (k, d))) ;
+                first by rewrite /CEP.eq_key /fst /CEP.SE.eq //.
+          apply SetoidList.In_InA ; first by exact Heqv_key.
+          rewrite CEP.Lemmas.P.of_list_1b // in Hfind_list.
+          apply SetoidList.findA_NoDupA in Hfind_list ;
+                last (by exact H6) ;
+                last (by exact Heqv_key0).
+          apply InA_In, Hfind_list.
+        - (* use H2 to show that PVM.find k conn_map = D_invalidated *)
+          rewrite (CEP.Lemmas.elements_o conn_map k).
+          generalize (SetoidList.findA_NoDupA (B := def_expr) Heqv_key0) ; intro.
+          specialize H11 with (eqA_dec := HiFP.PVSLemmas.P.FM.eq_dec) (l := CEP.elements conn_map) (a := k) (b := D_fexpr (Eref h)) (1 := CEP.elements_3w conn_map).
+          rewrite (proj1 H11).
+          * destruct H7 as [H7 _] ; move /andP : H7 => [/andP [_ /eqP H7] _].
+            apply H7.
+          * apply H2, SetoidList.InA_cons_hd.
+            by done.
+      + destruct (y == ic) eqn: Hyic.
+        - move /eqP : Hyic => Hyic ; rewrite Hyic.
+          destruct H7 as [H7 _] ; move /andP : H7 => [_ /eqP H7] ; rewrite H7.
+          destruct (PVM.find ic (CEP.Lemmas.P.of_list conn_map_list)) eqn: Hfind_list.
+          * specialize (H2 (ic, d)).
+            rewrite CEP.Lemmas.P.of_list_1b in Hfind_list ; last by apply H6.
+            apply SetoidList.findA_NoDupA in Hfind_list ;
+                  last (by apply H6) ; last by apply Heqv_key0.
+            apply SetoidList.InA_cons_tl with (y := (k, D_fexpr (Eref h))) in Hfind_list.
+            apply H2, CEP.elements_2, CEP.find_1 in Hfind_list.
+            by rewrite Hfind_list //.
+          * destruct (PVM.find ic conn_map) eqn: Hfind_map.
+            + apply CEP.find_2, CEP.elements_1 in Hfind_map.
+              apply H2, SetoidList.InA_cons in Hfind_map.
+              destruct Hfind_map as [Hfind_map|Hfind_map] ;
+                    first (by rewrite /PVM.eq_key_elt /PVM.Raw.Proofs.PX.eqke /fst -Hyic Hyk in Hfind_map ;
+                              destruct Hfind_map as [Hfind_map _] ; done).
+              rewrite CEP.Lemmas.P.of_list_1b in Hfind_list ; last by exact H6.
+              apply (SetoidList.findA_NoDupA Heqv_key0 ProdVarOrder.eq_dec ic d H6) in Hfind_map.
+              by rewrite Hfind_map // in Hfind_list.
+            + by reflexivity.
+        - destruct H7 as [_ H7].
+          specialize (H7 y).
+          rewrite mem_seq1 Hyk orFb mem_seq1 Hyic in H7.
+          rewrite -H7.
+          destruct (PVM.find y (CEP.Lemmas.P.of_list conn_map_list)) eqn: Hfind_list.
+          * specialize (H2 (y, d)).
+            rewrite CEP.Lemmas.P.of_list_1b in Hfind_list ; last by apply H6.
+            apply SetoidList.findA_NoDupA in Hfind_list ;
+                  last (by apply H6) ; last by apply Heqv_key0.
+            apply SetoidList.InA_cons_tl with (y := (k, D_fexpr (Eref h))) in Hfind_list.
+            apply H2, CEP.elements_2, CEP.find_1 in Hfind_list.
+            by rewrite Hfind_list //.
+          * destruct (PVM.find y conn_map) eqn: Hfind_map.
+            + apply CEP.find_2, CEP.elements_1 in Hfind_map.
+              apply H2, SetoidList.InA_cons in Hfind_map.
+              destruct Hfind_map as [Hfind_map|Hfind_map] ;
+                    first (by rewrite /PVM.eq_key_elt /PVM.Raw.Proofs.PX.eqke /fst Hyk in Hfind_map ;
+                              destruct Hfind_map as [Hfind_map _] ; done).
+              rewrite CEP.Lemmas.P.of_list_1b in Hfind_list ; last by exact H6.
+              apply (SetoidList.findA_NoDupA Heqv_key0 ProdVarOrder.eq_dec y d H6) in Hfind_map.
+              by rewrite Hfind_map // in Hfind_list.
+            + by reflexivity.
+Qed.
+
+
+Theorem ExpandBranches_Sem_ct :
 (* This theorem relates the connection maps generated by Sem_frag_stmts and ExpandBranch_funs. *)
 forall (ss old_def_ss : HiFP.hfstmt_seq) (vm_old vm_new vm_tmap : CEP.t vertex_type)
        (ct_old ct_new old_conn_map : CEP.t def_expr) (old_scope tmap : CEP.t ftype)
        (old_tmap_scope new_tmap_scope : CEP.t ftype * CEP.t ftype),
     stmts_have_fully_inferred_ground_types ss ->
     tmap_has_fully_inferred_ground_types old_tmap_scope.1 ->
-    submap old_scope old_tmap_scope.2 ->
-    submap old_tmap_scope.2 old_tmap_scope.1 ->
+    CEP.submap old_scope old_tmap_scope.2 ->
+    CEP.submap old_tmap_scope.2 old_tmap_scope.1 ->
     stmts_tmap old_tmap_scope ss vm_tmap = Some new_tmap_scope ->
-    submap new_tmap_scope.1 tmap ->
+    CEP.submap new_tmap_scope.1 tmap ->
     Sem_frag_stmts vm_old ct_old ss vm_new ct_new tmap ->
     CEP.Equal ct_old old_conn_map ->
        match ExpandBranch_funs ss old_def_ss old_conn_map old_scope with
@@ -1464,16 +2247,16 @@ forall (ss old_def_ss : HiFP.hfstmt_seq) (vm_old vm_new vm_tmap : CEP.t vertex_t
            CEP.Equal ct_new new_conn_map
        | None => True
        end
-with ExpandBranch_Sem :
+with ExpandBranch_Sem_ct :
 forall (s : HiFP.hfstmt) (old_def_ss : HiFP.hfstmt_seq) (vm_old vm_new vm_tmap : CEP.t vertex_type)
        (ct_old ct_new old_conn_map : CEP.t def_expr) (old_scope tmap : CEP.t ftype)
        (old_tmap_scope new_tmap_scope : CEP.t ftype * CEP.t ftype),
     stmt_has_fully_inferred_ground_types s ->
     tmap_has_fully_inferred_ground_types old_tmap_scope.1 ->
-    submap old_scope old_tmap_scope.2 ->
-    submap old_tmap_scope.2 old_tmap_scope.1 ->
+    CEP.submap old_scope old_tmap_scope.2 ->
+    CEP.submap old_tmap_scope.2 old_tmap_scope.1 ->
     stmt_tmap old_tmap_scope s vm_tmap = Some new_tmap_scope ->
-    submap new_tmap_scope.1 tmap ->
+    CEP.submap new_tmap_scope.1 tmap ->
     Sem_frag_stmt vm_old ct_old s vm_new ct_new tmap ->
     CEP.Equal ct_old old_conn_map ->
        match ExpandBranch_fun s old_def_ss old_conn_map old_scope with
@@ -1483,7 +2266,7 @@ forall (s : HiFP.hfstmt) (old_def_ss : HiFP.hfstmt_seq) (vm_old vm_new vm_tmap :
        | None => True
        end.
 Proof.
-* clear ExpandBranches_Sem.
+* clear ExpandBranches_Sem_ct.
   induction ss ; first by (unfold Sem_frag_stmts, ExpandBranch_funs ; intros ;
                            apply (CEP.Lemmas.Equal_trans (m' := ct_old)) ; last (by apply H6) ;
                            apply CEP.Lemmas.Equal_sym, H5).
@@ -1494,7 +2277,7 @@ Proof.
   move /andP : H => [H H7].
   simpl stmts_tmap in H3.
   destruct H5 as [vm' [ct' [H5 H8]]].
-  specialize (ExpandBranch_Sem h old_def_ss vm_old vm' vm_tmap ct_old ct' old_conn_map old_scope tmap old_tmap_scope).
+  specialize (ExpandBranch_Sem_ct h old_def_ss vm_old vm' vm_tmap ct_old ct' old_conn_map old_scope tmap old_tmap_scope).
   generalize (stmt_submap vm_tmap h old_tmap_scope.1 old_tmap_scope.2 H2) ; intro.
   rewrite -surjective_pairing in H9.
   specialize (ExpandBranch_stmt_tmap vm_tmap h old_tmap_scope.1)
@@ -1502,21 +2285,21 @@ Proof.
   rewrite -surjective_pairing in H10.
   destruct (stmt_tmap old_tmap_scope h vm_tmap) as [[tmap' scope']|] eqn: Htmap_scope' ; last by discriminate H3.
   specialize (H10 tmap' scope') with (1 := Logic.eq_refl).
-  specialize (ExpandBranch_Sem (tmap', scope') H H0 H1 H2 Logic.eq_refl) with (2 := H5) (3 := H6).
+  specialize (ExpandBranch_Sem_ct (tmap', scope') H H0 H1 H2 Logic.eq_refl) with (2 := H5) (3 := H6).
   destruct (ExpandBranch_fun h old_def_ss old_conn_map old_scope) as [[[temp_def_ss temp_conn_map] temp_scope]|] ;
         last by done.
   specialize (H10 temp_scope temp_def_ss temp_conn_map Logic.eq_refl H1 H).
   specialize (stmt_tmap_preserves_fully_inferred vm_tmap old_tmap_scope.1 old_tmap_scope.2 h H H0 H2) ; intro.
   rewrite -surjective_pairing Htmap_scope' in H11.
   specialize (IHss temp_def_ss vm' vm_new vm_tmap ct' ct_new temp_conn_map temp_scope tmap (tmap', scope') new_tmap_scope H7 H11 H10 (proj1 H9) H3 H4 H8).
-  apply IHss, ExpandBranch_Sem.
+  apply IHss, ExpandBranch_Sem_ct.
   simpl fst.
   generalize (stmts_submap vm_tmap ss tmap' scope' (proj1 H9)) ; intro.
   rewrite H3 in H12.
   destruct new_tmap_scope as [new_tmap new_scope].
-  apply (submap_trans new_tmap) ; last by apply H4.
-  apply H12.
-* clear ExpandBranch_Sem.
+  apply (CEP.Lemmas.submap_trans (proj1 (proj2 H12))).
+  apply H4.
+* clear ExpandBranch_Sem_ct.
   destruct s ; simpl ; try done ; intros.
   + (* Sskip *)
     rewrite -(proj2 H5) //.
@@ -1528,10 +2311,10 @@ Proof.
     rewrite -H7 in H3 ; clear newgt H7.
     destruct new_tmap_scope as [new_tmap new_scope].
     injection H3 ; clear H3 ; intros _ H3.
-    rewrite /fst -H3 /submap in H4.
-    specialize (H4 s).
+    rewrite /fst -H3 in H4.
+    specialize (H4 s (Gtyp gt)).
     rewrite CEP.Lemmas.find_add_eq in H4 ; last by rewrite /PVM.SE.eq //.
-    rewrite H4 /size_of_ftype add1n in H5.
+    rewrite H4 // /size_of_ftype add1n in H5.
     destruct H5 as [_ [_ [H5 H7]]].
     intro.
     destruct (y == s) eqn: Hys.
@@ -1583,10 +2366,10 @@ Proof.
           2: destruct (type_of_expr h1 old_tmap_scope.2) ; last by discriminate H3.
           1,2: injection H3 ; done.
     clear H3 ; rename H7 into H3.
-    rewrite /fst -H3 /submap in H4.
-    specialize (H4 s).
+    rewrite /fst -H3 in H4.
+    specialize (H4 s (Gtyp gt)).
     rewrite CEP.Lemmas.find_add_eq in H4 ; last by rewrite /PVM.SE.eq //.
-    rewrite H4 /size_of_ftype add1n in H5.
+    rewrite H4 // /size_of_ftype add1n in H5.
     destruct H5 as [_ [_ [_ [H7 [_ H5]]]]].
     intro.
     destruct (y == s) eqn: Hys.
@@ -1611,7 +2394,7 @@ Proof.
         right ; right ; move /ltP : H8 => H8 ; exact H8.
   + (* Snode *)
     destruct (type_of_expr h old_scope) as [[_ _]|] ; last by done.
-    generalize (submap_addl old_tmap_scope.1 tmap s) ; intro.
+    generalize (@CEP.Lemmas.submap_add_find_none _ old_tmap_scope.1 tmap s) ; intro.
     destruct (CEP.find s old_tmap_scope.1) ; first by discriminate H3.
     generalize (expr_preserves_fully_inferred old_tmap_scope.1 H0 h H) ; intro.
     generalize (type_of_expr_submap h old_tmap_scope.2 old_tmap_scope.1 H2) ; intro.
@@ -1622,37 +2405,18 @@ Proof.
     destruct new_tmap_scope as [new_tmap new_scope].
     injection H3 ; clear H3 ; intros _ H3.
     rewrite /fst -H3 in H4.
-    specialize (H7 (Gtyp gt) Logic.eq_refl H4).
+    specialize (H7 (Gtyp gt) H4 Logic.eq_refl).
     rewrite (H10 H7) in H5 ; clear p H10 H7.
-    destruct H5 as [_ [_ [H5 H7]]].
-    intro.
-    destruct (y == s) eqn: Hys.
-    - move /eqP : Hys => Hys ; rewrite Hys CEP.Lemmas.find_add_eq ; last by rewrite /PVM.SE.eq //.
-      replace (list_rhs_expr_p h (Gtyp gt)) with (Some [:: h]) in H7
-            by (destruct h ; done).
-      specialize (H7 N0).
-      rewrite add0n nat_of_binK -surjective_pairing // in H7.
-    - rewrite CEP.Lemmas.find_add_neq ; last by rewrite /PVM.SE.eq Hys //.
-      specialize (H5 y.1 y.2).
-      rewrite -surjective_pairing in H5.
-      move /eqP : Hys => Hys.
-      destruct (y.1 == s.1) eqn: Hys1 ; move /eqP : Hys1 => Hys1 ;
-            last by (rewrite -H5 ; last (by left ; exact Hys1) ;
-                     apply H6).
-      destruct (Nat.compare_spec y.2 s.2).
-      * specialize (injective_projections y s Hys1) ; intro.
-        rewrite -(nat_of_binK y.2) -(nat_of_binK s.2) H9 in H10.
-        rewrite H10 // in Hys.
-      * rewrite -H5 ; first (by apply H6).
-        right ; left ; move /ltP : H9 => H9 ; exact H9.
-      * rewrite -H5 ; first (by apply H6).
-        right ; right ; move /ltP : H9 => H9 ; exact H9.
+    destruct H5 as [_ [_ H5]].
+    apply CEP.Lemmas.Equal_trans with (m' := ct_old) ; last by exact H6.
+    apply CEP.Lemmas.Equal_sym, H5.
   + (* Sfcnct *)
     unfold ExpandBranch_connect.
     destruct h ; try (by done) ; last by (destruct h ; try done ; destruct h ; done).
     generalize (type_of_expr_submap h0 old_scope old_tmap_scope.2 H1) ; intro.
     specialize (H1 s).
     destruct (CEP.find s old_scope) as [ft_ref|] ; last by done.
+    specialize (H1 ft_ref Logic.eq_refl).
     destruct (type_of_expr h0 old_scope) as [[ft_expr p]|] ; last by done.
     destruct (connect_type_compatible false ft_ref ft_expr false) ; last by done.
     rewrite /type_of_ref H1 H7 in H3.
@@ -1665,12 +2429,12 @@ Proof.
     generalize (expr_preserves_fully_inferred old_tmap_scope.1 H0 h0 H) ; intro.
     rewrite H3 in H9.
     destruct ft_expr as [gt_expr| |] ; try by contradiction H9.
-    specialize (H2 s) ; rewrite H1 in H2.
-    specialize (H0 s) ; rewrite H2 in H0.
+    specialize (H2 s ft_ref) ; rewrite H1 in H2.
+    specialize (H0 s) ; rewrite H2 // in H0.
     destruct ft_ref as [gt_ref| |] ; try by contradiction H0.
-    specialize (H4 s) ; rewrite H2 in H4.
+    specialize (H4 s (Gtyp gt_ref)) ; rewrite H2 // in H4.
     simpl list_lhs_ref_p in H5.
-    rewrite /type_of_ref H4 H8 in H5.
+    rewrite /type_of_ref H4 // H8 in H5.
     replace (list_rhs_expr_p h0 (Gtyp gt_expr)) with (Some [:: h0]) in H5
           by (destruct h0 ; done).
     destruct h0.
@@ -1683,7 +2447,7 @@ Proof.
                       specialize (H5 0) ; simpl in H5 ;
                       rewrite N.add_0_r -surjective_pairing in H5 ;
                       move /eqP : Hys => Hys ;
-                      rewrite Hys H5 //).
+                      rewrite Hys (proj2 H5) //).
     1-6: rewrite CEP.Lemmas.find_add_neq ; last (by rewrite /PVM.SE.eq Hys //).
     1-6: destruct H5 as [_ H5].
     1-6: specialize (H5 y).
@@ -1714,7 +2478,7 @@ Proof.
     - rewrite CEP.Lemmas.find_add_eq ; last by (rewrite /PVM.SE.eq Hys //).
       move /eqP : Hys => Hys.
       rewrite Hys.
-      move /andP : H11 => [/eqP H11 _].
+      move /andP : H11 => [/andP [_ /eqP H11] _].
       rewrite N.add_0_r -surjective_pairing // in H11.
     - rewrite CEP.Lemmas.find_add_neq ; last (by rewrite /PVM.SE.eq Hys //).
       destruct (y == oc) eqn: Hyoc.
@@ -1730,15 +2494,16 @@ Proof.
     destruct h ; try (by done) ; last by (destruct h ; try done ; destruct h ; done).
     specialize (H1 s).
     destruct (CEP.find s old_scope) as [ft_ref|] ; last by done.
+    specialize (H1 ft_ref Logic.eq_refl).
     rewrite /type_of_ref H1 in H3.
     injection H3 ; clear H3 ; intro H3.
     rewrite -H3 in H4 ; clear new_tmap_scope H3.
-    specialize (H2 s) ; rewrite H1 in H2.
-    specialize (H4 s) ; rewrite H2 in H4.
+    specialize (H2 s ft_ref) ; rewrite H1 in H2.
+    specialize (H4 s ft_ref) ; rewrite H2 // in H4.
     simpl list_lhs_ref_p in H5.
-    rewrite H4 in H5.
+    rewrite H4 // in H5.
     specialize (H0 s).
-    rewrite H2 in H0.
+    rewrite H2 // in H0.
     destruct ft_ref as [gt_ref| |] ; try by contradiction H0.
     destruct H5 as [_ H5].
     intro.
@@ -1748,7 +2513,7 @@ Proof.
                       specialize (H5 0) ; simpl in H5 ;
                       rewrite N.add_0_r -surjective_pairing in H5 ;
                       move /eqP : Hys => Hys ;
-                      rewrite Hys H5 //).
+                      rewrite Hys (proj2 H5) //).
     rewrite CEP.Lemmas.find_add_neq ; last (by rewrite /PVM.SE.eq Hys //).
     destruct H5 as [_ H5].
     specialize (H5 y).
@@ -1760,23 +2525,23 @@ Proof.
     destruct (type_of_expr cond old_tmap_scope.2) ; last by discriminate H3.
     generalize (stmts_submap vm_tmap ss_true old_tmap_scope.1 old_tmap_scope.2 H2) ; intro.
     rewrite -(surjective_pairing) in H7.
-    assert (submap old_scope tmap).
-          apply (submap_trans old_tmap_scope.2) ; first by exact H1.
-          apply (submap_trans old_tmap_scope.1) ; first by exact H2.
+    assert (CEP.submap old_scope tmap).
+          apply (CEP.Lemmas.submap_trans H1).
+          apply (CEP.Lemmas.submap_trans H2).
           destruct (stmts_tmap old_tmap_scope ss_true vm_tmap) as [[tmap_true scope_true]|] ; last by discriminate H3.
-          generalize (submap_trans scope_true old_tmap_scope.2 tmap_true (proj2 (proj2 H7)) (proj1 H7)) ; intro.
+          generalize (CEP.Lemmas.submap_trans (proj2 (proj2 H7)) (proj1 H7)) ; intro.
           generalize (stmts_submap vm_tmap ss_false tmap_true old_tmap_scope.2 H8) ; intro.
           destruct (stmts_tmap (tmap_true, old_tmap_scope.2) ss_false vm_tmap) as [[tmap_false scope_false]|] ; last by discriminate H3.
-          apply (submap_trans tmap_true) ; first by apply H7.
-          apply (submap_trans tmap_false) ; first by apply H9.
+          apply (CEP.Lemmas.submap_trans (proj1 (proj2 H7))).
+          apply (CEP.Lemmas.submap_trans (proj1 (proj2 H9))).
           destruct new_tmap_scope as [new_tmap new_scope].
           injection H3 ; clear H3 ; intros _ H3.
           rewrite H3 //.
     generalize (type_of_expr_submap cond old_scope tmap H8) ; intro.
     destruct (type_of_expr cond old_scope) as [[[[[|[]]| | | | | |]| |] p]|] ; try by done.
-    generalize (ExpandBranches_Sem ss_true old_def_ss vm_old) ; intro.
+    generalize (ExpandBranches_Sem_ct ss_true old_def_ss vm_old) ; intro.
     specialize H10 with (vm_tmap := vm_tmap) (old_tmap_scope := old_tmap_scope).
-    move /andP : H => [Htrue Hfalse].
+    move /andP : H => [/andP [_ Htrue] Hfalse].
     generalize (stmts_tmap_preserves_fully_inferred vm_tmap ss_true old_tmap_scope.1 old_tmap_scope.2 Htrue H0 H2) ; intro.
     rewrite -surjective_pairing in H.
     destruct (stmts_tmap old_tmap_scope ss_true vm_tmap) as [[tmap_true scope_true]|] ; last by discriminate H3.
@@ -1785,51 +2550,148 @@ Proof.
     specialize (H10 vm_true ct_old ct_true old_conn_map old_scope tmap (tmap_true, scope_true) Htrue H0 H1 H2 Logic.eq_refl)
           with (2 := proj1 H5) (3 := H6).
     destruct (ExpandBranch_funs ss_true old_def_ss old_conn_map old_scope) as [[[true_def_ss true_conn_map] _]|] ; last by done.
-    assert (submap old_tmap_scope.2 tmap_true)
-          by (apply (submap_trans scope_true) ; apply H7).
-    specialize (ExpandBranches_Sem ss_false true_def_ss vm_true vm_new vm_tmap ct_old ct_false old_conn_map old_scope tmap (tmap_true, old_tmap_scope.2))
-          with (1 := Hfalse) (2 := H) (3 := H1) (4 := H11) (7 := proj1 (proj2 H5)) (8 := H6).
+    assert (CEP.submap old_tmap_scope.2 tmap_true)
+          by (apply (CEP.Lemmas.submap_trans (proj2 (proj2 H7)) (proj1 H7))).
+    specialize (ExpandBranches_Sem_ct ss_false true_def_ss vm_true vm_new vm_tmap (extend_map_with ct_old ct_true) ct_false (extend_map_with old_conn_map true_conn_map) old_scope tmap (tmap_true, old_tmap_scope.2))
+          with (1 := Hfalse) (2 := H) (3 := H1) (4 := H11) (7 := proj1 (proj2 H5)).
     generalize (stmts_submap vm_tmap ss_false tmap_true old_tmap_scope.2 H11) ; intro.
     destruct (stmts_tmap (tmap_true, old_tmap_scope.2) ss_false vm_tmap) as [[tmap_false scope_false]|] ; last by discriminate H3.
     destruct new_tmap_scope as [new_tmap new_scope].
     injection H3 ; clear H3 ; intros _ H3.
     rewrite -H3 /fst in H4.
-    specialize (ExpandBranches_Sem (tmap_false, scope_false) Logic.eq_refl H4).
-    destruct (ExpandBranch_funs ss_false true_def_ss old_conn_map old_scope) as [[[false_def_ss false_conn_map] _]|] ; last by done.
+    specialize (ExpandBranches_Sem_ct (tmap_false, scope_false) Logic.eq_refl H4).
+    destruct (ExpandBranch_funs ss_false true_def_ss (extend_map_with old_conn_map true_conn_map) old_scope) as [[[false_def_ss false_conn_map] _]|] ; last by done.
     destruct H5 as [_ [_ H5]].
     intro.
     rewrite (H5 y) CEP.Lemmas.map2_1bis ; last by rewrite /helper_tf //.
     rewrite CEP.Lemmas.map2_1bis ; last by rewrite /Swhen_map2_helper //.
-    rewrite (ExpandBranches_Sem y).
-    assert (submap tmap_true tmap)
-          by (apply (submap_trans tmap_false) ; last (by exact H4) ;
-              apply H12).
+    assert (CEP.submap tmap_true tmap)
+          by (apply (CEP.Lemmas.submap_trans (proj1 (proj2 H12)) H4)).
     specialize (H10 H13).
+    assert (CEP.Equal (extend_map_with ct_old ct_true)
+                      (extend_map_with old_conn_map true_conn_map))
+          by (intro ; specialize (H6 y0) ; specialize (H10 y0) ;
+              rewrite /extend_map_with CEP.Lemmas.map2_1bis // CEP.Lemmas.map2_1bis // H6 H10 //).
+    specialize (ExpandBranches_Sem_ct H14).
+    rewrite (ExpandBranches_Sem_ct y).
     rewrite (H10 y) /Swhen_map2_helper /helper_tf.
     destruct (CEP.find y true_conn_map) as [[]|] ; destruct (CEP.find y false_conn_map) as [[]|] ; reflexivity.
 Qed.
 
-(*
-forall (vm_old vm_new : CEP.t vertex_type) (pp : seq HiFP.hfport) (ss : HiFP.hfstmt_seq),
-    ports_have_fully_inferred_ground_types pp ->
+
+Lemma Sem_frag_stmts_uncomponent :
+(* This lemma is the core of the correctness theorem.
+   It shows that the split in (component_stmts_of ss) and a connection map
+   can be undone. *)
+forall (ss : HiFP.hfstmt_seq)
+       (vm_old : CEP.t vertex_type) (ct_old : CEP.t def_expr) (vm_new : CEP.t vertex_type) (ct_new : CEP.t def_expr) (tmap : CEP.t ftype)
+       (old_def_ss : HiFP.hfstmt_seq)
+       (old_scope : CEP.t ftype)
+       (ss_conn_map : CEP.t def_expr) (new_scope : CEP.t ftype),
     stmts_have_fully_inferred_ground_types ss ->
-    match port_stmts_tmap pp ss vm with
-    | Some tmap =>
-        match ExpandPort_fun pp with
-        | Some (port_conn_map, _) =>
-            match ExpandBranch_funs ss old_def_ss ct_old old_scope with
-            | Some (def_ss, new_conn_map, new_scope) =>
-                exists (vm' vm_new : CEP.t ftype),
-                              Sem_frag_ports (CEP.empty vertex_type) (CEP.empty def_expr) pp vm' port_conn_map tmap
-                           /\ Sem_frag_stmts vm' port_conn_map ss vm_new conn_map
-                        (* /\ vm_new is the extension of vm' with def_ss *)
-            | None => True
-            end
-        | None => True
-        end
-    | None => True
-    end.
-*)
+    tmap_has_fully_inferred_ground_types tmap ->
+    ct_has_fully_inferred_ground_types ct_old ->
+    vm_and_ct_compatible vm_old ct_old ->
+    (* ct_old and old_scope fit together -> *)
+    CEP.submap old_scope tmap ->
+    ExpandBranch_funs ss old_def_ss ct_old old_scope =
+        Some (Qcat old_def_ss (component_stmts_of ss), ss_conn_map, new_scope) ->
+    Sem_frag_stmts vm_old ct_old (Qcat (component_stmts_of ss) (CEP.fold helper_connect ss_conn_map (Qnil ProdVarOrder.T))) vm_new ct_new tmap ->
+        Sem_frag_stmts vm_old ct_old ss vm_new ct_new tmap
+with Sem_frag_stmt_uncomponent :
+forall (s : HiFP.hfstmt)
+       (vm_old : CEP.t vertex_type) (ct_old : CEP.t def_expr) (vm_new : CEP.t vertex_type) (ct_new : CEP.t def_expr) (tmap : CEP.t ftype)
+       (old_def_ss : HiFP.hfstmt_seq)
+       (old_scope : CEP.t ftype)
+       (s_conn_map : CEP.t def_expr) (new_scope : CEP.t ftype),
+    stmt_has_fully_inferred_ground_types s ->
+    tmap_has_fully_inferred_ground_types tmap ->
+    ct_has_fully_inferred_ground_types ct_old ->
+    vm_and_ct_compatible vm_old ct_old ->
+    (* ct_old and old_scope fit together -> *)
+    CEP.submap old_scope tmap ->
+    ExpandBranch_fun s old_def_ss ct_old old_scope =
+        Some (Qcat old_def_ss (component_stmt_of s), s_conn_map, new_scope) ->
+    Sem_frag_stmts vm_old ct_old (Qcat (component_stmt_of s) (CEP.fold helper_connect s_conn_map (Qnil ProdVarOrder.T))) vm_new ct_new tmap ->
+        Sem_frag_stmt vm_old ct_old s vm_new ct_new tmap.
+Proof.
+* clear Sem_frag_stmts_uncomponent.
+  induction ss ; simpl ; intros.
+  + (* induction base *)
+    injection H4 ; clear H4 ; intros _ H4 _.
+    rewrite -H4 in H5 ; clear ss_conn_map H4.
+    generalize (helper_connect_Sem ct_old vm_old ct_old vm_new ct_new tmap H0 H1 H5) ; intro.
+    split ; first by apply H4.
+    destruct H4 as [_ H4].
+    intro ; rewrite H4 /extend_defined_map_with CEP.Lemmas.map2_1bis //.
+    destruct (CEP.find y ct_old) as [[| |]|] ; by reflexivity.
+  + (* induction step *)
+    rename h into s.
+    move /andP : H => H.
+    (* We want the following commutative diagram:
+
+           vm_old/ct_old ---------------------------.
+                 |                                   \ by Sem_frag_stmt_uncomponent
+                 |                                    \ it is possible to
+                 | comp s                              \ change this to s.
+                 |                                      \
+                 v                   conn s              v
+       vm_after_s/ct_after_comp_s -----------> vm_after_s/ct_after_s ---------------------.
+                 |                                       |                                 \ by induction hypothesis
+                 |                                       |                                  \ it is possible to
+                 | comp ss                               | comp ss                           \ change this to ss.
+                 |                                       |                                    \
+                 v                      conn s           v                   conn ss           v
+           vm_new/ct_after_comp_s_ss ------------> vm_new/ct_after_conn_s -------------> vm_new/ct_new
+
+       In this diagram, we have the leftmost and the bottom path by the assumptions of the theorem.
+       (Connection maps are the same as the resulting ct,
+       so we can use the result of ExpandBranch_fun(s) as ct,
+       see ExpandBranch_Sem_ct.
+       Perhaps we will have to change that, so that helper_connect will only generate connect statements
+       for things that actually have been connected in the code translated by ExpandBranch_funs.)
+       Perhaps, we may have to construct ct_after_conn_s.
+       To use the induction hypothesis, we also need to construct ct_after_conn_s; that is:
+          extend_defined_map_with conn_map_s ct_after_comp_s_ss. *)
+    specialize (Sem_frag_stmt_uncomponent s vm_old ct_old)
+          with (old_def_ss := old_def_ss) (old_scope := old_scope) (tmap := tmap).
+    specialize (ExpandBranch_component) with (scope := old_scope) (s := s) (def_ss := old_def_ss) (conn_map := ct_old) ; intro.
+    destruct (ExpandBranch_fun s old_def_ss ct_old old_scope) as [[[def_ss_after_s ct_after_s] scope_after_s]|] eqn: Hexpand_s ;
+          last by discriminate H4.
+    specialize (H6 def_ss_after_s ct_after_s scope_after_s Logic.eq_refl).
+    subst def_ss_after_s.
+    specialize Sem_frag_stmt_uncomponent with (s_conn_map := ct_after_s) (new_scope := scope_after_s)
+               (1 := proj1 H) (2 := H0) (3 := H1) (4 := H2).
+    specialize (ExpandBranch_components) with (scope := scope_after_s) (ss := ss) (def_ss := Qcat old_def_ss (component_stmt_of s)) (conn_map := ct_after_s) ; intro.
+    destruct (ExpandBranch_funs ss (Qcat old_def_ss (component_stmt_of s)) ct_after_s scope_after_s) as [[[new_def_ss ct_new'] new_scope']|] eqn: Hexpand_ss ;
+          last by discriminate H4.
+    specialize (H6 new_def_ss ct_new' new_scope' Logic.eq_refl).
+    subst new_def_ss.
+    injection H4 ; clear H4 ; intros H4 H6 _.
+    subst new_scope' ss_conn_map.
+    apply Sem_frag_stmts_cat in H5.
+    destruct H5 as [vm_new' [ct_after_comp_s_ss [H5 H7]]].
+    assert (tmap_has_fully_inferred_ground_types old_scope).
+          intro.
+          specialize (H3 v) ; specialize (H0 v).
+          destruct (CEP.find v old_scope) ; last by trivial.
+          rewrite (H3 f) // in H0.
+    generalize (ExpandBranch_fun_preserves_fully_inferred (Qcat old_def_ss (component_stmt_of s)) ct_after_s old_scope s old_def_ss ct_old scope_after_s
+                H4 (proj1 H) H1 Hexpand_s) ; intro H8.
+    generalize (ExpandBranch_funs_preserves_fully_inferred ss (Qcat old_def_ss (component_stmt_of s)) ct_after_s scope_after_s
+                (Qcat old_def_ss (Qcat (component_stmt_of s) (component_stmts_of ss))) ct_new' new_scope
+                (proj1 H8) (proj2 H) (proj2 H8)) ; intro H9.
+    rewrite -Qcat_assoc in H9 ; specialize (H9 Hexpand_ss).
+    generalize (helper_connect_Sem ct_new' vm_new' ct_after_comp_s_ss vm_new ct_new tmap
+                H0 (proj2 H9) H7) ; intro H10.
+    apply Sem_frag_stmts_cat in H5.
+    destruct H5 as [vm_after_s [ct_after_comp_s [H5 H6]]].
+    exists vm_after_s, ct_after_s.
+    admit.
+* clear Sem_frag_stmt_uncomponent.
+  admit.
+Admitted.
+
 
 (* What would a theorem to relate expandBranch_funs with Sem_frag_stmts look like?
    We need to find an inductive formulation.
@@ -1846,19 +2708,276 @@ forall (vm_old vm_new : CEP.t vertex_type) (pp : seq HiFP.hfport) (ss : HiFP.hfs
 
 Ultimately we want:
    Given ExpandBranch_funs ss old_def_ss ct_old old_scope = Some (def_ss, new_conn_map, new_scope)
-     and Sem_frag_stmts vm_old ct_old (Qcat def_ss (... new_conn_map)) vm_new ct_new tmap,
+     and Sem_frag_stmts vm_old ct_old (Qcat def_ss (CEP.fold helper_connect conn_map (Some (Qnil ProdVarOrder.T)))) vm_new ct_new tmap,
    then Sem_frag_stmts vm_old ct_old ss vm_new ct_new tmap.
 *)
 
+(* The point is perhaps rather:
+in the induction step of the correctness theorem,
+we have something like
+old graph -> one statement -> temp graph -> sequence of statements -> new graph
 
+We know (as induction hypothesis) that for the sequence of statements, we can transform
+from a split (component/connection) to a single sequence of combined statements.
+
+We also know (as the other induction hypothesis) that the one statement
+can be transformed from a split (component/connection) to a single statement.
+
+We have then to show that the connection part of the one statement
+can be moved through the sequence of statements.
+This is basically done by Sem_frag_stmts_component_Equal.
+
+In the corresponding theorem for single statements,
+the only complex case is the Swhen statement.
+
+*)
+
+Lemma ExpandBranches_correct :
+forall (vm_new : CEP.t vertex_type) (ct_new : CEP.t def_expr) (new_tmap_scope : CEP.t ftype * CEP.t ftype)
+       (ss : HiFP.hfstmt_seq) (vm_old : CEP.t vertex_type) (ct_old : CEP.t def_expr) (old_def_ss : HiFP.hfstmt_seq) (old_conn_map new_conn_map : CEP.t def_expr)
+       (old_scope new_scope : CEP.t ftype) (old_tmap_scope : CEP.t ftype * CEP.t ftype),
+        tmap_has_fully_inferred_ground_types old_tmap_scope.1 ->
+        (* ExpandPort_fun pp = Some (old_conn_map, old_scope) -> *)
+        (* submap old_scope tmap ->*)
+        vm_and_ct_compatible vm_old ct_old ->
+        CEP.Equal ct_old old_conn_map ->
+        stmts_have_fully_inferred_ground_types ss ->
+        CEP.submap old_tmap_scope.2 old_tmap_scope.1 ->
+        stmts_tmap old_tmap_scope ss vm_new = Some new_tmap_scope ->
+        ExpandBranch_funs ss old_def_ss old_conn_map old_scope =
+              Some (Qcat old_def_ss (component_stmts_of ss), new_conn_map, new_scope) ->
+        Sem_frag_stmts vm_old ct_old (Qcat (component_stmts_of ss) (CEP.fold helper_connect new_conn_map (Qnil ProdVarOrder.T))) vm_new ct_new new_tmap_scope.1 ->
+            Sem_frag_stmts vm_old ct_old ss vm_new ct_new new_tmap_scope.1.
+Proof.
+intros.
+apply Sem_frag_stmts_cat in H6.
+destruct H6 as [vm_temp [ct_temp [H6 H7]]].
+generalize (Sem_frag_stmts_component ss vm_old ct_old vm_temp ct_temp new_tmap_scope.1 H0 H6) ; intro.
+generalize (stmts_tmap_preserves_fully_inferred vm_new ss old_tmap_scope.1 old_tmap_scope.2 H2 H H3) ; intro.
+rewrite -surjective_pairing H4 in H9.
+destruct new_tmap_scope as [new_tmap_s new_t_scope].
+generalize (helper_connect_Sem new_conn_map vm_temp ct_temp vm_new ct_new new_tmap_s H9) ; intro.
+specialize H10 with (2 := H7).
+(* Here follows an older attempt to prove ExpandBranches_correct
+   by induction on ss.  The problem is that connect statements
+   would need a very intricate treatment, depending on whether
+   the statement is the last or not.
+   (For this, it would have been easier to define statement sequences
+   right-recursive, using Qrcons.)
+induction ss as [|s ss].
+* simpl ; intros.
+  (* use a lemma that says:
+  CEP.fold helper_connect new_conn_map (Some (Qnil ProdVarOrder.T)) = Some new_conn_ss ->
+  Sem_frag_stmts vm_old ct_old new_conn_ss vm_new ct_new tmap ->
+     CEP.Equal vm_old vm_new /\ CEP.Equal (extend_map_with new_conn_map ct_old) ct_new. *)
+  admit.
+* simpl ; intros.
+  generalize (stmt_submap vm_new s old_tmap_scope.1 old_tmap_scope.2 H2) ; intro.
+  rewrite -surjective_pairing in H7.
+  destruct (stmt_tmap old_tmap_scope s vm_new) as [temp_tmap_scope|] eqn: Hstmt_tmap ; last by discriminate H3.
+  rewrite (surjective_pairing temp_tmap_scope) in H7.
+  generalize (stmts_submap vm_new ss temp_tmap_scope.1 temp_tmap_scope.2 (proj1 H7)) ; intro.
+  rewrite -surjective_pairing in H8.
+  destruct (stmts_tmap temp_tmap_scope ss vm_new) as [new_tmap_scope'|] eqn: Hstmts_tmap ; last by discriminate H3.
+  injection H3 ; clear H3 ; intro H3.
+  rewrite H3 in H8, Hstmts_tmap ; clear H3 new_tmap_scope'.
+  rewrite (surjective_pairing new_tmap_scope) in H8.
+  (* Let's just do two examples statements to try how it works... *)
+  destruct s ; try by done.
+  + (* Sskip *)
+    simpl.
+    exists vm_old, ct_old.
+    split ; first by (split ; reflexivity).
+    move /andP : H1 => [_ H1].
+    simpl stmt_tmap in Hstmt_tmap.
+    injection Hstmt_tmap ; clear Hstmt_tmap ; intro Hstmt_tmap.
+    rewrite -Hstmt_tmap in H7, H8, Hstmts_tmap ; clear Hstmt_tmap temp_tmap_scope.
+    simpl in H4.
+    simpl Qcat in H6.
+    by apply (IHss vm_old ct_old old_def_ss new_conn_ss old_conn_map new_conn_map old_scope new_scope old_tmap_scope
+                   H H0 H1 H2 Hstmts_tmap H4 H5 H6).
+  + (* Swire -- a component statement *)
+    move /andP : H1 => [H1s H1ss].
+    simpl stmt_has_fully_inferred_ground_types in H1s.
+    destruct f as [gt| |] ; try rewrite // in H1s.
+    unfold ExpandBranch_fun in H4.
+    rewrite -Qcat_rcons in H4.
+    simpl Sem_frag_stmts in H6.
+    destruct H6 as [vm' [ct' H6]].
+    unfold stmt_tmap in Hstmt_tmap.
+    destruct (CEP.find s old_tmap_scope.1) eqn: Hold_tmap_scope ; first by discriminate Hstmt_tmap.
+    generalize (fully_inferred_does_not_change gt s vm_new H1s) ; intro.
+    destruct (code_type_find_vm_widths (Gtyp gt) s vm_new) as [[[gt'| |] p]|] ; try by done.
+    rewrite -H1 in Hstmt_tmap ; clear gt' H1.
+    injection Hstmt_tmap ; clear Hstmt_tmap ; intro Hstmt_tmap.
+    rewrite -Hstmt_tmap in Hstmts_tmap, H7, H8 ; clear temp_tmap_scope Hstmt_tmap.
+    simpl fst in H7, H8 ; simpl snd in H7, H8.
+    generalize (proj1 (proj2 H8) s) ; intro.
+    rewrite CEP.Lemmas.find_add_eq in H1 ; last by rewrite /PVM.SE.eq eq_refl //.
+    rewrite (H1 (Gtyp gt)) // in H6.
+    specialize (IHss (CEP.add s (Wire gt) vm_old) (CEP.add s D_undefined old_conn_map) (Qrcons old_def_ss (Swire (var:=ProdVarOrder.T) s (Gtyp gt)))
+                     new_conn_ss (CEP.add s D_undefined old_conn_map)
+                     new_conn_map (CEP.add s (Gtyp gt) old_scope) new_scope
+                     (CEP.add s (Gtyp gt) old_tmap_scope.1, CEP.add s (Gtyp gt) old_tmap_scope.2))
+                with (2 := CEP.Lemmas.Equal_refl (CEP.add s D_undefined old_conn_map)) (3 := H1ss)
+                     (4 := proj1 H7) (5 := Hstmts_tmap) (6 := H4) (7 := H5).
+    simpl fst in IHss ; simpl snd in IHss.
+    exists (CEP.add s (Wire gt) vm_old), (CEP.add s D_undefined old_conn_map).
+    split.
+    - admit.
+    - apply IHss.
+      * intro ; destruct (v == s) eqn: Hvs.
+        + rewrite CEP.Lemmas.find_add_eq ; last by rewrite /PVM.SE.eq Hvs //.
+          by exact H1s.
+        + rewrite CEP.Lemmas.find_add_neq ; last by rewrite /PVM.SE.eq Hvs //.
+          by apply H.
+      * (* almost proj2 H6 *)
+        apply (Sem_frag_stmts_Equal (Qcat (component_stmts_of ss) new_conn_ss)
+                                    vm' (CEP.add s (Wire gt) vm_old)
+                                    ct' (CEP.add s D_undefined old_conn_map)
+                                    vm_new vm_new ct_new ct_new new_tmap_scope.1 new_tmap_scope.1)
+                               with (3 := CEP.Lemmas.Equal_refl vm_new) (4 := CEP.Lemmas.Equal_refl ct_new)
+                                    (5 := CEP.Lemmas.Equal_refl new_tmap_scope.1) (6 := proj2 H6).
+        + clear -H6 ; destruct H6 as [[H0 [H1 _]] _].
+          intro.
+          destruct (y == s) eqn: Hys.
+          - rewrite CEP.Lemmas.find_add_eq ; last by rewrite /PVM.SE.eq Hys //.
+            specialize (H0 0).
+            move /eqP : Hys => Hys.
+            rewrite /list_rhs_type_p /List.nth_error add0n nat_of_binK -surjective_pairing -Hys in H0.
+            by apply H0.
+          - rewrite CEP.Lemmas.find_add_neq ; last by rewrite /PVM.SE.eq Hys //.
+            specialize (H1 y.1 y.2).
+            rewrite -surjective_pairing /size_of_ftype add1n in H1.
+            rewrite H1 //.
+            destruct (N.eq_dec y.1 s.1) as [H|H] ; last (left ; exact H).
+            right.
+            destruct (Nat.compare_spec y.2 s.2) ;
+                  first (by specialize (injective_projections y s H) ; intro ;
+                            rewrite -(nat_of_binK y.2) -(nat_of_binK s.2) H2 in H3 ;
+                            specialize (H3 Logic.eq_refl) ;
+                            rewrite H3 eq_refl // in Hys) ;
+                  move /ltP : H2 => H2.
+            * left  ; exact H2.
+            * right ; exact H2.
+        + clear -H6 H0 ; destruct H6 as [[_ [_ [H1 H2]]] _].
+          intro.
+          destruct (y == s) eqn: Hys.
+          - rewrite CEP.Lemmas.find_add_eq ; last by rewrite /PVM.SE.eq Hys //.
+            specialize (H2 0).
+            move /eqP : Hys => Hys.
+            rewrite /list_rhs_type_p /List.nth_error add0n nat_of_binK -surjective_pairing -Hys in H2.
+            by apply H2.
+          - rewrite CEP.Lemmas.find_add_neq ; last by rewrite /PVM.SE.eq Hys //.
+            specialize (H1 y.1 y.2).
+            rewrite -surjective_pairing /size_of_ftype add1n in H1.
+            rewrite -H1 ; first by apply H0.
+            destruct (N.eq_dec y.1 s.1) as [H|H] ; last (left ; exact H).
+            right.
+            destruct (Nat.compare_spec y.2 s.2) ;
+                  first (by specialize (injective_projections y s H) ; intro ;
+                            rewrite -(nat_of_binK y.2) -(nat_of_binK s.2) H3 in H4 ;
+                            specialize (H4 Logic.eq_refl) ;
+                            rewrite H4 eq_refl // in Hys) ;
+                  move /ltP : H3 => H3.
+            * left  ; exact H3.
+            * right ; exact H3.
+  + (* Sreg -- should be similar to Swire *)
+    admit.
+  + (* Snode -- should be similar to Swire *)
+    admit.
+  + (* Sfcnct *)
+    simpl stmt_has_fully_inferred_ground_types in H1.
+    move /andP : H1 => [H1s H1ss].
+    simpl Qcat in H4, H6.
+    simpl ExpandBranch_fun in H4.
+    unfold ExpandBranch_connect in H4.
+    destruct h ; try (by discriminate H4) ;
+          last by destruct h ; try (by discriminate H4) ;
+                  destruct h ; by discriminate H4.
+    simpl stmt_tmap in Hstmt_tmap.
+    destruct (CEP.find s old_tmap_scope.2) ; last by discriminate Hstmt_tmap.
+    destruct (type_of_expr h0 old_tmap_scope.2) ; last by discriminate Hstmt_tmap.
+    injection Hstmt_tmap ; clear Hstmt_tmap ; intro Hstmt_tmap.
+    rewrite -Hstmt_tmap in H7 H8 Hstmts_tmap ; clear temp_tmap_scope Hstmt_tmap.
+    (* Perhaps we need here that ft_ref is fully inferred?
+       Then we would also need to assume tmap_has_fully_inferred_ground_types old_scope. *)
+    destruct (CEP.find s old_scope) as [ft_ref|] ; last by discriminate H4.
+    destruct (type_of_expr h0 old_scope) as [[ft_expr _]|] ; last by discriminate H4.
+    destruct (connect_type_compatible false ft_ref ft_expr false) ; last by discriminate H4.
+    specialize (IHss vm_old (CEP.add s (D_fexpr h0) ct_old) old_def_ss new_conn_ss
+                     (CEP.add s (D_fexpr h0) old_conn_map) (CEP.remove ??? new_conn_map) old_scope new_scope old_tmap_scope
+                     H) with (2 := H1ss) (3 := H2) (4 := Hstmts_tmap) (5 := H4) (6 := H5).
+
+This does not work properly as it is now.
+We need to change new_conn_map:
+If this "Sfcnct ref expr" statement is the last connect,
+then one should remove the assignment to ref from new_conn_map in the induction hypothesis.
+If there is another connect statement, the later one prevails.
+
+We may resolve this by a lemma.
+Something like:
+a) In a correct program (without repeated definitions of components),
+   a later component statement will not overwrite old connect statements,
+   i.e. if all statements in ss are component statements,
+        then CEP.submap ct_old ct_new.
+   see Lemma Sem_frag_stmts_component.
+
+b) To get the semantics of the connect map correct:
+   we have something like (CEP.Equal ct_new (extend_map_with new_conn_map ct_old)).
+   see Lemma helper_connect_Sem?
+
+Then the connect statement's effect ends up in (CEP.add s (D_fexpr h0) ct_old).
+
+Another idea:
+First split the module into component and non-component statements
+(without changing the structure).
+The non-component statements only consist of
+- Sfcnct
+- Sinvalid
+- Swhen
+Then show that a program consisting of these does not change under ExpandWhens.
+This may be easier because the domain of the connect map never changes.
+
+Aha! Is that a way out? Not have a connect map that is undefined
+for some components that have no connection statement in the branch?
+
+Or rather try to formulate another inductive statement like:
+
+the connect map of a branch (Qcons (Sfcnct ...) ss) and
+the connect map of ss have this relation:
+CEP.Equal (connect_map_of (Qcons (Sfcnct (Eid s) expr) ss))
+          (extend_expr_map_with (connect_map_of ss) (CEP.add s (D_fexpr expr) (CEP.empty def_expr)))
+
+and extend_expr_map_with takes into account validif expressions,
+allowing for partial extension if ss did not define something in every subbranch.
+
+Definition extend_expr_map_with_helper (ex1 ex2 : option def_expr) : option def_expr :=
+match ex1, ex2 with
+| None, _ => ex2
+| Some D_fexpr expr1, Some D_fexpr expr2 =>
+    (recursively go through expr1 and replace any (validif condition e1)
+     with (mux condition e1 expr2)
+     may require something like validifnot expressions
+     to see whether the mux should be positive or negative).
+| _, _ => ex1
+end.
+
+Definition extend_expr_map_with (m1 m2 : CEP.t def_expr) : CEP.t def_expr :=
+CEP.map2 extend_expr_map_with_helper m1 m2.
+*)
+Admitted.
+
+
+(*
 Lemma ExpandBranches_correct :
 forall (vm : CEP.t vertex_type) (ct : CEP.t def_expr)
        (ss old_def_ss def_ss old_conn_ss new_conn_ss : HiFP.hfstmt_seq)
-       (old_conn_map conn_map ct' : CEP.t def_expr) (old_scope tmap : CEP.t ftype)
+       (old_conn_map conn_map ct' : CEP.t def_expr) (old_scope temp_scope tmap : CEP.t ftype)
        (vm' : CEP.t vertex_type),
 (* perhaps tmap_has_fully_inferred_ground_types tmap -> *)
-(exists temp_scope, ExpandBranch_funs ss old_def_ss old_conn_map old_scope = Some ((Qcat old_def_ss def_ss), conn_map, temp_scope)) ->
-def_ss = component_stmts_of ss ->
+ExpandBranch_funs ss old_def_ss old_conn_map old_scope = Some ((Qcat old_def_ss def_ss), conn_map, temp_scope) ->
+(*def_ss = component_stmts_of ss -> -- follows from ExpandBranches_component *)
 CEP.fold helper_connect conn_map (Some (Qnil ProdVarOrder.T)) = Some new_conn_ss ->
 Sem_frag_stmts vm' ct' (Qcat def_ss (Qcat old_conn_ss new_conn_ss)) vm ct tmap ->
 (* vm' contains the component definitions in old_def_ss and old_conn_map -> *)
@@ -1868,10 +2987,10 @@ Sem_frag_stmts vm' ct' (Qcat def_ss (Qcat old_conn_ss new_conn_ss)) vm ct tmap -
 with ExpandBranch_correct :
 forall (vm : CEP.t vertex_type) (ct : CEP.t def_expr)
        (s : HiFP.hfstmt) (old_def_ss def_ss old_conn_ss new_conn_ss : HiFP.hfstmt_seq)
-       (old_conn_map conn_map ct' : CEP.t def_expr) (old_scope tmap : CEP.t ftype)
+       (old_conn_map conn_map ct' : CEP.t def_expr) (old_scope temp_scope tmap : CEP.t ftype)
        (vm' : CEP.t vertex_type),
-(exists temp_scope, ExpandBranch_fun s old_def_ss old_conn_map old_scope = Some ((Qcat old_def_ss def_ss), conn_map, temp_scope)) ->
-def_ss = component_stmt_of s ->
+ExpandBranch_fun s old_def_ss old_conn_map old_scope = Some ((Qcat old_def_ss def_ss), conn_map, temp_scope) ->
+(*def_ss = component_stmt_of s -> -- follows from ExpandBranch_component *)
 CEP.fold helper_connect conn_map (Some (Qnil ProdVarOrder.T)) = Some new_conn_ss ->
 Sem_frag_stmts vm' ct' (Qcat def_ss (Qcat old_conn_ss new_conn_ss)) vm ct tmap ->
 (* vm' contains the component definitions in old_def_ss and old_conn_map -> *)
@@ -1880,15 +2999,24 @@ Sem_frag_stmts vm' ct' (Qcat def_ss (Qcat old_conn_ss new_conn_ss)) vm ct tmap -
    Sem_frag_stmt vm' ct' s vm ct tmap.
 Proof.
 * clear ExpandBranches_correct.
-  induction ss.
-  + simpl.
-    intros.
-    rewrite H0 in H, H2 ; clear def_ss H0.
-    simpl Qcat in H2 ; rewrite Qcats0 in H.
-    destruct H ; injection H ; clear H ; intros _ H ; clear x.
-    clear old_conn_map H.
+  induction ss ; simpl ; intros.
+  + injection H ; clear H ; intros _ H _ ; clear temp_scope.
+    rewrite -H in H1 ; clear conn_map H.
+    rewrite H0 in H2 ; simpl Qcat in H2.
+    (* simpl.
+      intros.
+      rewrite H0 in H, H2 ; clear def_ss H0.
+      simpl Qcat in H2 ; rewrite Qcats0 in H.
+      destruct H ; injection H ; clear H ; intros _ H ; clear x.
+      clear old_conn_map H. *)
+    admit.
+  + admit.
+* clear ExpandBranch_correct.
+  induction s ; simpl ; intros.
+  + (* Sskip *)
+    rewrite CEP.fold_1 in H1.
 Admitted.
-
+*)
 
 Definition ExpandWhens_fun (m : HiFP.hfmodule) : option HiFP.hfmodule :=
 (* expand whens in module m *)
@@ -1898,10 +3026,7 @@ match m with
     | Some (port_conn_map, port_scope) =>
         match ExpandBranch_funs ss (Qnil ProdVarOrder.T) port_conn_map port_scope with
         | Some (def_ss, conn_map, _) =>
-            match CEP.fold helper_connect conn_map (Some (Qnil ProdVarOrder.T)) with
-            | Some conn_ss => Some (FInmod v pp (Qcat def_ss conn_ss))
-            | None => None
-            end
+            Some (FInmod v pp (Qcat def_ss (CEP.fold helper_connect conn_map (Qnil ProdVarOrder.T))))
         | None => None
         end
     | None => None
@@ -1936,53 +3061,97 @@ generalize (ExpandPort_correct vm pp Hpp) ;
       intro.
 destruct (ExpandPort_fun pp) as [[port_conn_map port_scope]|] eqn: Hport ; last by discriminate.
 destruct (ExpandBranch_funs ss (Qnil ProdVarOrder.T) port_conn_map port_scope) as [[[def_ss conn_map] scope]|] eqn: Hexpand ; last by discriminate H0.
-destruct (CEP.fold helper_connect conn_map (Some (Qnil ProdVarOrder.T))) as [conn_ss|] eqn: Hfold ; last by discriminate H0.
 injection H0 ; clear H0 ; intro.
 rewrite -H0 in H1 ; clear H0 m'.
 unfold Sem in H1 ; unfold Sem.
+unfold ports_stmts_tmap in H1 ; unfold ports_stmts_tmap.
 generalize (ports_tmap_preserves_fully_inferred vm pp Hpp) ;
       intro.
 destruct (ports_tmap pp vm) as [pmap|] ; last by trivial.
-generalize (stmts_tmap_components vm ss pmap pmap pmap (submap_refl pmap) (submap_refl pmap) (submap_refl pmap)) ;
+generalize (stmts_tmap_components vm ss pmap pmap pmap (CEP.Lemmas.submap_refl pmap) (CEP.Lemmas.submap_refl pmap) (CEP.Lemmas.submap_refl pmap)) ;
       intro.
 generalize (ExpandBranch_components ss (Qnil ProdVarOrder.T) port_conn_map port_scope
             def_ss conn_map scope Hexpand) ;
       intro ;
       unfold Qcat in H3.
-rewrite stmts_tmap_cat H3 in H1.
+rewrite stmts_tmap_cat H3 in H1 ; rewrite H3 in Hexpand ; clear def_ss H3.
 generalize (ExpandBranch_funs_checks_scopes ss pmap pmap pmap vm
-            Hss H0 (submap_refl pmap) (submap_refl pmap) (submap_refl pmap)) ;
+            Hss H0 (CEP.Lemmas.submap_refl pmap) (CEP.Lemmas.submap_refl pmap) (CEP.Lemmas.submap_refl pmap)) ;
       intro.
-specialize H4 with (old_def_ss := (Qnil ProdVarOrder.T))
-                   (old_conn_map := port_conn_map) (old_scope := port_scope).
+specialize H3 with (old_def_ss := (Qnil ProdVarOrder.T))
+                   (old_conn_map := port_conn_map) (old_scope := port_scope)
+                   (3 := CEP.Lemmas.Equal_submap (CEP.Lemmas.Equal_sym H)).
 generalize (stmts_submap vm (component_stmts_of ss) pmap pmap
-            (submap_refl pmap)) ;
+            (CEP.Lemmas.submap_refl pmap)) ;
+      intro.
+generalize (components_preserves_fully_inferred ss Hss) ;
+      intro.
+generalize (stmts_tmap_preserves_fully_inferred vm (component_stmts_of ss) pmap pmap H5 H0 (CEP.Lemmas.submap_refl pmap)) ;
       intro.
 destruct (stmts_tmap (pmap, pmap) (component_stmts_of ss) vm) as [[tmap' scope2]|] ; last by contradiction H1.
 destruct (stmts_tmap (pmap, pmap) ss vm) as [[tmap scope1]|] ;
-      last by (rewrite Hexpand in H4 ; discriminate H4 ; try done ;
+      last by (rewrite Hexpand in H3 ; discriminate H3 ; try done ;
                intro ; specialize (H v0) ; rewrite H ;
                destruct (CEP.find v0 port_scope) ; done).
-clear H4.
-destruct H2 as [H2' H2] ; rewrite -H2' in H1 H5 ; clear H2' tmap'.
-generalize (stmts_tmap_components vm conn_ss tmap scope2 scope2
-            (proj1 H5) (proj1 H5) (submap_refl scope2)) ;
+clear H3.
+destruct H2 as [H2' H2] ; rewrite -H2' in H1 H4 H6 ; clear H2' tmap'.
+generalize (stmts_tmap_components vm (CEP.fold helper_connect conn_map
+                    (Qnil ProdVarOrder.T)) tmap scope2 scope2
+            (proj1 H4) (proj1 H4) (CEP.Lemmas.submap_refl scope2)) ;
       intro.
-destruct (stmts_tmap (tmap, scope2) conn_ss vm) as [[tmap' scope2']|] ; last by contradiction H1.
-generalize (proj2 (fold_connect_components conn_map) (Qnil ProdVarOrder.T)) ;
+destruct (stmts_tmap (tmap, scope2) (CEP.fold helper_connect conn_map
+                    (Qnil ProdVarOrder.T)) vm) as [[tmap' scope2']|] ; last by contradiction H1.
+generalize (fold_connect_components conn_map (Qnil ProdVarOrder.T)) ;
       intro.
-rewrite Hfold in H6 ; simpl component_stmts_of in H6.
-rewrite H6 /stmts_tmap in H4 ; clear H6.
-destruct H4 as [H4 _] ; rewrite H4 in H1 ; clear H4 tmap'.
+simpl component_stmts_of in H7.
+rewrite H7 /stmts_tmap in H3 ; clear H7.
+destruct H3 as [H3 _] ; rewrite H3 in H1 ; clear H3 tmap' scope2'.
 split ; first by (apply H1).
 destruct H1 as [_ [vm' [ct' H1]]].
 exists vm', ct'.
 split ; first by apply H1.
-clear scope2'.
-destruct H5 as [_ [H5 _]].
+destruct H4 as [_ [H4 _]].
 clear H2 scope2 scope1.
-replace pmap with port_scope in H0, H5 by (admit).
-clear H pmap.
+rename H0 into H0'.
+assert (H0 : tmap_has_fully_inferred_ground_types port_scope).
+      clear -H H0'.
+      intro.
+      specialize (H v) ; specialize (H0' v).
+      destruct (CEP.find v pmap) as [[gt| |]|] ;
+            try (by done) ; rewrite -H //.
+rename H4 into H4'.
+assert (H4 : CEP.submap port_scope tmap).
+      clear -H H4'.
+      intro.
+      specialize (H k) ; specialize (H4' k).
+      destruct (CEP.find k port_scope) as [ft|] ; last by done.
+      rewrite H // in H4'.
+clear H0' H4' H pmap.
+destruct H1 as [_ H1].
+(* Now use something like a Sem_frag_stmts_cat lemma,
+   looking at the state of vm'' and ct'' between (component_stmts_of ss) and conn_ss.
+   We can prove that
+   * Sem_frag_stmts vm' ct' (component_stmts_of ss) vm'' ct'' tmap
+     + sets vm essentially to the same as Sem_frag_stmts vm' ct' ss vm ct tmap.
+     + sets ct'' to all default values.
+   * Sem_frag_stmts vm'' ct'' conn_ss vm ct tmap
+     + does not really change vm, we have CEP.Equal vm'' vm
+     + sets ct to the same values as ss
+       (this may need a more intricate proof!)
+
+Or use another proof idea:
+induction by ss.
+If the first statement of ss is a component statement,
+it moves to the first part of H1's Sem_frag_stmts.
+
+If the first statement of ss is a connection statement,
+then ExpandBranch_funs moves its effect to conn_map,
+and CEP.fold helper_connect moves its effect to conn_ss.
+
+---
+
+Requires actually a mutual induction over statement sequences and statements.
+*)
 
 
 
@@ -2016,3 +3185,17 @@ Sem_frag_stmts vm_old ct_old (Qcat (components ss) (connections ss)) vm ct
 
 So we need to strengthen Hexpand so we can use this correspondence!
 *)
+Admitted.
+
+(* Example *)
+
+Definition test_ports0 := [:: Finput  (var := ProdVarOrder.T) (1%num, N0) (Gtyp (Fuint 10)) ;
+                              Foutput (var := ProdVarOrder.T) (2%num, N0) (Gtyp (Fuint 10))].
+Definition test_stmts0 := Qcons (Snode (var := ProdVarOrder.T) (3%num, N0) (Eref (Eid (var := ProdVarOrder.T) (1%num, N0))))
+                         (Qcons (Sfcnct (Eid (var := ProdVarOrder.T) (2%num, N0)) (Econst ProdVarOrder.T (Fuint 1) [:: true]))
+                         (Qcons (Sfcnct (Eid (var := ProdVarOrder.T) (2%num, N0)) (Eref (Eid (var := ProdVarOrder.T) (3%num, N0))))
+                                (Qnil _))).
+
+Definition test_mod := FInmod (var := ProdVarOrder.T) (101%num, N0) test_ports0 test_stmts0.
+
+Compute (ExpandWhens_fun test_mod).
